\documentclass[11pt]{article}
\newcommand{\PSCHAIN}{..}
\input{../prepend_PS_chain}
\newcommand{\rootdir}{\PSCHAIN}
\input{\PSCHAIN/includes/includes}


\begin{document}
\doublespacing
\MOONSTITLE
\maketitle

\section{LSA Governing equations}

The LSA governing equations (derived elsewhere) are
\begin{equation}\begin{aligned}
\PD_t v = -\frac{1}{\rho}\PD_y P - \frac{1}{\rho \M} B_x^0 \PD_y B_x^{1} \\
\PD_t w = -\frac{1}{\rho}\PD_z P - \frac{1}{\rho \M} B_x^0 \PD_z B_x^{1} \\
\theta + \PD_t B_x^{1} = \frac{1}{\sigma \M} (\PD_{yy} B_x^{1}+\PD_{zz} B_x^{1}) \\
\PD_y v + \PD_z w = 0  \\
\end{aligned} \end{equation}

\section{Exponential form}
We have 4 equations and 4 unknowns.
\begin{equation}\begin{aligned}
\PD_t v = -\frac{1}{\rho}\PD_y P - \frac{1}{\rho \M} B_x^0 \PD_y B_x^{1} \\
\PD_t w = -\frac{1}{\rho}\PD_z P - \frac{1}{\rho \M} B_x^0 \PD_z B_x^{1} \\
\theta + \PD_t B_x^{1} = \frac{1}{\sigma \M} (\PD_{yy} B_x^{1}+\PD_{zz} B_x^{1}) \\
\PD_y v + \PD_z w = 0  \\
\end{aligned} \end{equation}
Assuming a solution of the form
\begin{equation}\begin{aligned}
v = \hat{v} e^{i\alpha y} e^{i\beta z} e^{\lambda t} \\
w = \hat{w} e^{i\alpha y} e^{i\beta z} e^{\lambda t} \\
P = \hat{P} e^{i\alpha y} e^{i\beta z} e^{\lambda t} \\
B_x^1 = \hat{B_x^1} e^{i\alpha y} e^{i\beta z} e^{\lambda t} \\
\end{aligned} \end{equation}
And multiplying by $\rho$, we have
\begin{equation}\begin{aligned}
\rho \lambda \hat{v} = -i \alpha \hat{P} - \frac{1}{\M} B_x^0 \PD_y B_x^{1} \\
\rho \lambda \hat{w} = -i \beta  \hat{P} - \frac{1}{\M} B_x^0 \PD_z B_x^{1} \\
\end{aligned} \end{equation}
Solving for $B_x^1$, we have

\begin{equation}\begin{aligned}
\theta + \lambda \hat{B_x^{1}} = \frac{1}{\sigma \M} (-\alpha^2 \hat{B_x^{1}}-\beta^2 \hat{B_x^{1}} ) \\
\sigma \M \theta + \sigma \M \lambda \hat{B_x^{1}} = -\alpha^2 \hat{B_x^{1}}-\beta^2 \hat{B_x^{1}} \\
(\alpha^2 +\beta^2 + \sigma \M \lambda ) \hat{B_x^{1}} = -\sigma \M \theta \\
\hat{B_x^{1}} = - \frac{\sigma \M \theta}{\alpha^2 +\beta^2 + \sigma \M \lambda} \\
\end{aligned} \end{equation}

\begin{equation}\begin{aligned}
\rho \lambda \hat{v} = -i \alpha \hat{P} - \frac{1}{\M} B_x^0 \PD_y B_x^{1} \\
\rho \lambda \hat{w} = -i \beta  \hat{P} - \frac{1}{\M} B_x^0 \PD_z B_x^{1} \\
\theta + \lambda \hat{B_x^{1}} = \frac{1}{\sigma \M} (-\alpha^2 \hat{B_x^{1}}-\beta^2 \hat{B_x^{1}} ) \\
\sigma \M \theta + \sigma \M \lambda \hat{B_x^{1}} = -\alpha^2 \hat{B_x^{1}}-\beta^2 \hat{B_x^{1}} \\
(\alpha^2 +\beta^2 + \sigma \M \lambda ) \hat{B_x^{1}} = -\sigma \M \theta \\
\hat{B_x^{1}} = - \frac{\sigma \M \theta}{\alpha^2 +\beta^2 + \sigma \M \lambda} \\
\alpha \hat{v} + \beta \hat{w} = 0  \\
\end{aligned} \end{equation}

Canceling pressure and solving for $\hat{v}$, we have
\begin{equation}\begin{aligned}
\hat{w} = - \frac{\alpha}{\beta} \hat{v} \\
-\rho \lambda (\frac{\alpha}{\beta} \hat{v}) = -i\beta \hat{P} - \frac{1}{\M} B_x^0 \PD_z B_x^{1} \\
-\rho \lambda (\frac{\alpha^2}{\beta^2} \hat{v}) = -i\alpha \hat{P} - \frac{\alpha}{\beta} \frac{1}{\M} B_x^0 \PD_z B_x^{1} \\
\rho \lambda (\frac{\alpha^2}{\beta^2} \hat{v}) = i\alpha \hat{P} + \frac{\alpha}{\beta} \frac{1}{\M} B_x^0 \PD_z B_x^{1} \\
\rho \lambda \hat{v} = -i\alpha \hat{P} - \frac{1}{\M} B_x^0 \PD_y B_x^{1} \\
\rho \lambda (\frac{\alpha^2}{\beta^2} \hat{v}) + \rho \lambda \hat{v} = \frac{\alpha}{\beta} \frac{1}{\M} B_x^0 \PD_z B_x^{1} - \frac{1}{\M} B_x^0 \PD_y B_x^{1} \\
\rho \lambda \left(1 + \frac{\alpha^2}{\beta^2} \right) \hat{v} = \frac{B_x^0}{\M} \left(\frac{\alpha}{\beta} \PD_z B_x^{1} - \PD_y B_x^{1} \right) \\
\end{aligned} \end{equation}


\end{document}