\documentclass[11pt]{article}
\newcommand{\PSCHAIN}{..}
\input{../prepend_PS_chain}
\newcommand{\rootdir}{\PSCHAIN}
\input{\PSCHAIN/includes/includes}


\begin{document}
\doublespacing
\MOONSTITLE
\maketitle

\section{Governing equations}
The dimensionless momentum and induction equations are
\begin{equation}\begin{aligned}
\PD_t u_i+u_j\PD_j u_i = -\PD_i p+ \frac{1}{Re} \PD_{jj} u_i + Al (B_j \PD_j B_i - \tfrac{1}{2} \PD_i B_j B_j) \\
\PD_t B_i + \PD_t B_i^0 = \frac{1}{Re_m} \PD_{jj} B_i - \PD_j (u_j B_i - u_i B_j)
\end{aligned} \end{equation}
Remove magnetic pressure
\begin{equation}\begin{aligned}
\PD_t u_i+u_j\PD_j u_i = -\PD_i p+ \frac{1}{Re} \PD_{jj} u_i + Al B_j \PD_j B_i \\
\PD_t B_i + \PD_t B_i^0 = \frac{1}{Re_m} \PD_{jj} B_i - \PD_j (u_j B_i - u_i B_j)
\end{aligned} \end{equation}
Expanding equations yields
\small
\begin{equation}\begin{aligned}
\PD_t u+ u\PD_x u + v\PD_y u + w\PD_z u = -\PD_x p+ \frac{1}{Re} (\PD_{xx} u+\PD_{yy} u+\PD_{zz} u) + Al (B_x \PD_x B_x + B_y \PD_y B_x + B_z \PD_z B_x) \\
\PD_t v+ u\PD_x v + v\PD_y v + w\PD_z v = -\PD_y p+ \frac{1}{Re} (\PD_{xx} v+\PD_{yy} v+\PD_{zz} v) + Al (B_x \PD_x B_y + B_y \PD_y B_y + B_z \PD_z B_y) \\
\PD_t w+ u\PD_x w + v\PD_y w + w\PD_z w = -\PD_z p+ \frac{1}{Re} (\PD_{xx} w+\PD_{yy} w+\PD_{zz} w) + Al (B_x \PD_x B_z + B_y \PD_y B_z + B_z \PD_z B_z) \\
\PD_t B_x + \PD_t B_x^0 = \frac{1}{Re_m} (\PD_{xx} B_x + \PD_{yy} B_x+\PD_{zz} B_x)                         - \PD_y (v B_x - u B_y) - \PD_z (w B_x - u B_z) \\
\PD_t B_y + \PD_t B_y^0 = \frac{1}{Re_m} (\PD_{xx} B_y + \PD_{yy} B_y+\PD_{zz} B_y) - \PD_x (u B_y - v B_x)                         - \PD_z (w B_y - v B_z) \\
\PD_t B_z + \PD_t B_z^0 = \frac{1}{Re_m} (\PD_{xx} B_z + \PD_{yy} B_z+\PD_{zz} B_z) - \PD_x (u B_z - w B_x) - \PD_y (v B_z - w B_y)                         \\
\end{aligned} \end{equation}
\normalsize
Assuming:
\begin{itemize}\setlength\itemsep{-1em}
	\item $\PD_x=0$ for all variables but pressure
\end{itemize}
We have
\begin{equation}\begin{aligned}
\PD_t u+ v\PD_y u + w\PD_z u = -\PD_x p+ \frac{1}{Re} (\PD_{yy} u+\PD_{zz} u) + Al (B_y \PD_y B_x + B_z \PD_z B_x) \\
\PD_t v+ v\PD_y v + w\PD_z v = -\PD_y p+ \frac{1}{Re} (\PD_{yy} v+\PD_{zz} v) + Al (B_y \PD_y B_y + B_z \PD_z B_y) \\
\PD_t w+ v\PD_y w + w\PD_z w = -\PD_z p+ \frac{1}{Re} (\PD_{yy} w+\PD_{zz} w) + Al (B_y \PD_y B_z + B_z \PD_z B_z) \\
\PD_t B_x + \PD_t B_x^0 = \frac{1}{Re_m} (\PD_{yy} B_x+\PD_{zz} B_x) - \PD_y (v B_x - u B_y) - \PD_z (w B_x - u B_z) \\
\PD_t B_y + \PD_t B_y^0 = \frac{1}{Re_m} (\PD_{yy} B_y+\PD_{zz} B_y)                         - \PD_z (w B_y - v B_z) \\
\PD_t B_z + \PD_t B_z^0 = \frac{1}{Re_m} (\PD_{yy} B_z+\PD_{zz} B_z) - \PD_y (v B_z - w B_y)                         \\
\end{aligned} \end{equation}
Assuming:
\begin{itemize}\setlength\itemsep{-1em}
	\item $\PD_t B_x^0$ = constant
	\item $B_y^0 = 0$
	\item $B_z^0 = $ uniform and constant
	\item $v = 0$
	\item $w = 0$
\end{itemize}
We have
\begin{equation}\begin{aligned}
\PD_t u = -\PD_x p + \frac{1}{Re} (\PD_{yy} u+\PD_{zz} u) + Al B_z^0 \PD_z B_x^1 \\
\PD_t B_x^1 + \PD_t B_x^0 = \frac{1}{Re_m} (\PD_{yy} B_x^1+\PD_{zz} B_x^1) + B_z^0 \PD_z u \\
\end{aligned} \end{equation}

\end{document}