\documentclass[11pt]{article}
\newcommand{\PSCHAIN}{..}
\input{../prepend_PS_chain}
\newcommand{\rootdir}{\PSCHAIN}
\input{\PSCHAIN/includes/includes}

\newcommand{\HALF}{\frac{1}{2}}

\begin{document}
\doublespacing
\MOONSTITLE
\maketitle

\section{ODE Solution}
Our decoupled, transformed governing equations are then:
\begin{equation}\begin{aligned}
C = \frac{1}{\M \sqrt{\mu \sigma}} \\
D = B_y^0 \sqrt{\frac{\sigma}{\mu}} \\
F = \frac{1}{\mu} \PD_x p \\
X = u + C B_x \\
Y = u - C B_x \\
X'' + D X' = F \\
Y'' - D Y' = F \\
u   = \frac{1}{2}  (X+Y) \\
B_x = \frac{1}{2C} (X-Y) \\
\end{aligned} \end{equation}

The general solution to these ODEs, using Wolfram Alpha, is
\begin{equation}\begin{aligned}
X = \frac{c_1}{D} e^{-D y} + \frac{F}{D} y + c_2  \\
Y = \frac{c_3}{D} e^{+D y} - \frac{F}{D} y + c_4  \\
\end{aligned} \end{equation}
Returning to our primitive variables to apply BCs, we have
\begin{equation}\begin{aligned}
u & = \frac{1}{2} (X+Y) \\
  & = \frac{1}{2} \left( \frac{c_1}{D} e^{-D y} + \frac{F}{D} y + c_2+\frac{c_3}{D} e^{+D y} - \frac{F}{D} y + c_4 \right) \\
  & = \frac{1}{2D} ( c_1 e^{-D y} + F y + D c_2 + c_3 e^{+D y} - F y + D c_4 ) \\
  & = \frac{1}{2D} ( c_1 e^{-D y} + D c_2 + c_3 e^{+D y} + D c_4 ) \\
\end{aligned} \end{equation}
And
\begin{equation}\begin{aligned}
B_x & = \frac{1}{2C} (X-Y) \\
    & = \frac{1}{2C} \left(\frac{c_1}{D} e^{-D y} + \frac{F}{D} y + c_2 - \frac{c_3}{D} e^{+D y} + \frac{F}{D} y - c_4\right) \\
    & = \frac{1}{2CD} (c_1 e^{-D y} + F y + D c_2 - c_3 e^{+D y} + F y - D c_4) \\
    & = \frac{1}{2CD} (c_1 e^{-D y} + D c_2 - c_3 e^{+D y} - D c_4 + 2F y) \\
\end{aligned} \end{equation}

\subsection{Particular solution}

Applying BCs, we have
\begin{equation}\begin{aligned}
u(-a)   = 0 & = \frac{1}{2D} ( c_1 e^{-D (-a)} + D c_2 + c_3 e^{+D (-a)} + D c_4) = 0 \\
u(+a)   = 0 & = \frac{1}{2D} ( c_1 e^{-D (+a)} + D c_2 + c_3 e^{+D (+a)} + D c_4) = 0 \\
B_x(-a) = 0 & = \frac{1}{2CD} (c_1 e^{-D (-a)} + D c_2 - c_3 e^{+D (-a)} - D c_4) + 2 F (-a)= 0 \\
B_x(+a) = 0 & = \frac{1}{2CD} (c_1 e^{-D (+a)} + D c_2 - c_3 e^{+D (+a)} - D c_4) + 2 F (+a)= 0 \\
\end{aligned} \end{equation}
So,
\begin{equation}\begin{aligned}
c_1 e^{+D a} + D c_2 + c_3 e^{-D a} + c_4 D & = 0 \\
c_1 e^{-D a} + D c_2 + c_3 e^{+D a} + c_4 D & = 0 \\
c_1 e^{+D a} + D c_2 - c_3 e^{-D a} - c_4 D & = +2 F a \\
c_1 e^{-D a} + D c_2 - c_3 e^{+D a} - c_4 D & = -2 F a \\
\end{aligned} \end{equation}
Using Matlab:
\begin{verbatim}
clc; close all; clear all
syms D a F
A = [exp(+D*a) D +exp(-D*a) +D;
     exp(-D*a) D +exp(+D*a) +D;
     exp(+D*a) D -exp(-D*a) -D;
     exp(-D*a) D -exp(+D*a) -D]
b = [0;0;2*F*a;-2*F*a]
c = inv(A)*b
r = latex(simplify(c))
test_1 = c(1) - c(3)
test_2 = c(2) - c(4)
\end{verbatim}
The solution was found to be:
\begin{equation}\begin{aligned}
c = \left(\begin{array}{c} \frac{2\, F\, a\, \mathrm{e}^{D\, a}}{\mathrm{e}^{2\, D\, a} - 1}\\ -\frac{F\, a\, \left(\mathrm{e}^{2\, D\, a} + 1\right)}{D\, \left(\mathrm{e}^{2\, D\, a} - 1\right)}\\ \frac{2\, F\, a\, \mathrm{e}^{D\, a}}{\mathrm{e}^{2\, D\, a} - 1}\\ -\frac{F\, a\, \left(\mathrm{e}^{2\, D\, a} + 1\right)}{D\, \left(\mathrm{e}^{2\, D\, a} - 1\right)} \end{array}\right) \\
\end{aligned} \end{equation}

Put slightly differently, we have
\begin{equation}\begin{aligned}
c_1  = c_3 =  \frac{Fa}{\sinh(Da)} \\
c_2  = c_4 = -\frac{Fa}{D} \frac{\cosh(Da)}{\sinh(Da)} \\
\end{aligned} \end{equation}

Therefore, our particular solution is
\small
\begin{equation}\begin{aligned}
u   & = \frac{1}{2D}  \left(\frac{Fa}{\sinh(Da)} e^{-D y} - D \frac{Fa}{D} \frac{\cosh(Da)}{\sinh(Da)} + \frac{Fa}{\sinh(Da)} e^{+D y} - D \frac{Fa}{D} \frac{\cosh(Da)}{\sinh(Da)} \right) \\
B_x & = \frac{1}{2DC} \left(\frac{Fa}{\sinh(Da)} e^{-D y} - D \frac{Fa}{D} \frac{\cosh(Da)}{\sinh(Da)} - \frac{Fa}{\sinh(Da)} e^{+D y} + D \frac{Fa}{D} \frac{\cosh(Da)}{\sinh(Da)} + 2F y \right) \\
\end{aligned} \end{equation}
Double check:
\normalsize
Simplifying velocity, we have
\begin{equation}\begin{aligned}
u   & = \frac{1}{2D}  \left(\frac{Fa}{\sinh(Da)} e^{-D y} - D \frac{Fa}{D} \frac{\cosh(Da)}{\sinh(Da)} + \frac{Fa}{\sinh(Da)} e^{+D y} - D \frac{Fa}{D} \frac{\cosh(Da)}{\sinh(Da)} \right) \\
    & = \frac{Fa}{2D \sinh(Da)}  \left(e^{-D y} - \cosh(Da) + e^{+D y} - \cosh(Da) \right) \\
    & = \frac{Fa}{2D \sinh(Da)}  \left(2 \cosh(Dy) - 2 \cosh(Da) \right) \\
    & = \frac{Fa}{D} \frac{\cosh(Da)}{\sinh(Da)}  \left( \frac{\cosh(Dy)}{\cosh(Da)}  - 1 \right) \\
\end{aligned} \end{equation}

The magnetic field is then
\begin{equation}\begin{aligned}
B_x & = \frac{1}{2DC} \left(\frac{Fa}{\sinh(Da)} e^{-D y} - D \frac{Fa}{D} \frac{\cosh(Da)}{\sinh(Da)} - \frac{Fa}{\sinh(Da)} e^{+D y} + D \frac{Fa}{D} \frac{\cosh(Da)}{\sinh(Da)} + 2F y \right) \\
    & = \frac{Fa}{2DC} \frac{1}{\sinh(Da)} \left(e^{-D y} - e^{+D y} + 2 \frac{y}{a} \sinh(Da) \right) \\
    & = \frac{Fa}{2DC} \frac{1}{\sinh(Da)} \left(-2\sinh(Dy) + 2 \frac{y}{a} \sinh(Da) \right) \\
    & = \frac{Fa}{DC} \left(-\frac{\sinh(Dy)}{\sinh(Da)} + \frac{y}{a} \right) \\
    & = \frac{Fa}{DC} \left(\frac{y}{a} - \frac{\sinh(Dy)}{\sinh(Da)}\right) \\
\end{aligned} \end{equation}

\subsection{Summary}

Our final solution is then
\begin{equation}\begin{aligned}
C   & = \frac{1}{\M \sqrt{\mu \sigma}} \\
D   & = B_y^0 \sqrt{\frac{\sigma}{\mu}} \\
F   & = \frac{1}{\mu} \PD_x p \\
u   & = \frac{Fa}{D} \frac{\cosh(Da)}{\sinh(Da)}  \left( \frac{\cosh(Dy)}{\cosh(Da)}  - 1 \right) \\
B_x & = \frac{Fa}{DC} \left(\frac{y}{a} - \frac{\sinh(Dy)}{\sinh(Da)}\right) \\
\end{aligned} \end{equation}

Noting the Hartmann number, we have
\begin{equation}\begin{aligned}
Ha  & = Da = a B_y^0 \sqrt{\frac{\sigma}{\mu}} \\
C   & = \frac{1}{\M \sqrt{\mu \sigma}} \\
F   & = \frac{1}{\mu} \PD_x p \\
u   & = \frac{Fa^2}{Ha} \frac{\cosh(Ha)}{\sinh(Ha)}  \left( \frac{\cosh(Ha \frac{y}{a} )}{\cosh(Ha)}  - 1 \right) \\
B_x & = \frac{Fa^2}{CHa} \left(\frac{y}{a} - \frac{\sinh(Ha \frac{y}{a})}{\sinh(Ha)}\right) \\
\end{aligned} \end{equation}

\begin{verbatim}
clc; clear all; close all;
D = 2;
F = 2;
a = 20;
C = 2;
y = linspace(-a,a);
Ha = D*a;
Hay = Ha*y/a;
u = F*a^2/Ha*cosh(Ha)/sinh(Ha)*(cosh(Hay)/cosh(Ha)-1);
B_x = F*a^2/Ha*(y/a - sinh(Hay)/sinh(Ha));
plot(y,u,y,B_x)
xlabel('y')
legend('u','B_x')
title('Hartmann Flow')
\end{verbatim}

\end{document}