\documentclass[11pt]{article}
\newcommand{\PSCHAIN}{..}
\input{../prepend_PS_chain}
\newcommand{\rootdir}{\PSCHAIN}
\input{\PSCHAIN/includes/includes}


\begin{document}
\doublespacing
\MOONSTITLE
\maketitle

\section{Solving for the Undetermined Coefficients}
Our decoupled equations are
\begin{equation}\begin{aligned}
\PD_t X - H X'' - DE X'  = (- EC -G)\\
\PD_t Y - H Y'' + DE Y'  = (+ EC -G)\\
\end{aligned} \end{equation}
With transformations
\begin{equation}\begin{aligned}
X = u + E B_x \\
Y = u - E B_x \\
E = \sqrt{\frac{A}{D}} \\
\end{aligned} \end{equation}
And inverse transformations
\begin{equation}\begin{aligned}
u   = \frac{1}{2} \left( X + Y \right) \\
B_x = \frac{1}{2E} \left( X - Y \right) \\
E = \sqrt{\frac{A}{D}} = \sqrt{\frac{1}{\rho \M}} \\
\end{aligned} \end{equation}
\begin{equation}\begin{aligned}
G = \frac{1}{\rho}\PD_x p, \qquad
H = \nu, \qquad
A = \frac{1}{\rho \M} B_z^0, \qquad
C = \PD_t B_x^0, \qquad
K = \frac{1}{\sigma \M}, \qquad
D = B_z^0, \qquad
\end{aligned} \end{equation}

\section{Solution prep}
First, let's introduce a variable so that we can solve both systems simultaneously. Let $\kappa = 1$ for the $X$ equation, and $\kappa = -1$ for the $Y$ equation.
\begin{equation}\begin{aligned}
	\PD_t \MAC X - H \MAC X'' - DE \kappa \MAC X'  = (- \kappa EC -G) \\
\end{aligned} \end{equation}
\section{Solution procedure}
First, let's decompose the solution into homogeneous and non-homogeneous:
\begin{equation}\begin{aligned}
	\MAC X = \MAC X_h + \MAC X_n, \\
\end{aligned} \end{equation}
where the homogeneous solution satisfies
\begin{equation}\begin{aligned}
	\PD_t \MAC X_h - H \MAC X_h'' - DE \kappa \MAC X_h'  = 0 \\
\end{aligned} \end{equation}
Assuming the homogeneous solution is separable ($\MAC X_h(z,t) = F(z)Q(t)$), we have
\begin{equation}\begin{aligned}
	F\dot{Q} - HQF'' - \kappa DEQF' = 0 \\
\end{aligned} \end{equation}
Dividing by $FQ$ yields
\begin{equation}\begin{aligned}
	\frac{\dot{Q}}{Q} = H \frac{F''}{F} + \kappa DE \frac{F'}{F} = \text{constant} = -\gamma \\
\end{aligned} \end{equation}
\subsection{Spatial solution}
Let's solve the RHS equation:
\begin{equation}\begin{aligned}
	H F'' + \kappa DE F' = -F \gamma \\
	F'' + \frac{\kappa DE}{H} F' = -\frac{F}{H} \gamma \\
\end{aligned} \end{equation}
Let's assume $F(z) = e^{i\alpha z}$, to get
\begin{equation}\begin{aligned}
	H F'' + \kappa DE F' = - F \gamma \\
	-\alpha^2 + i \frac{\kappa DE}{H} \alpha = - \frac{1}{H} \gamma \\
	-\alpha^2 + i\frac{\kappa DE}{H} \alpha + \frac{1}{H} \gamma = 0  \\
	\alpha^2 - i\frac{\kappa DE}{H} \alpha - \frac{1}{H} \gamma = 0  \\
	\alpha = i \frac{\kappa DE}{2H} \pm \frac{1}{2} \sqrt{\left(\frac{i \kappa DE}{H}\right)^2 - \frac{4}{H} \gamma} \\
	\alpha = i \frac{\kappa DE}{2H} \pm \frac{i}{2} \sqrt{\left(\frac{\kappa DE}{H}\right)^2 + \frac{4}{H} \gamma} \\
\end{aligned} \end{equation}
From this, we may write
\begin{equation}\begin{aligned}
	\alpha_1 + \alpha_2 = i \frac{\kappa DE}{H} \\
	\alpha_1 - \alpha_2 = i \sqrt{\left(\frac{DE}{H}\right)^2 + \frac{4}{H} \gamma} \\
\end{aligned} \end{equation}

So, we have
\begin{equation}\begin{aligned}
	F(z) = c_1 e^{\alpha_1 z} + c_2 e^{\alpha_2 z} \\
\end{aligned} \end{equation}
Applying BC ($F(0) = 0$)
\begin{equation}\begin{aligned}
	F(0) = & c_1 + c_2 = 0 \\
	     = & c_2 =-c_1  \\
\end{aligned} \end{equation}
Yields
\begin{equation}\begin{aligned}
	F(z) = c_1 (e^{\alpha_1 z} - e^{\alpha_2 z}) \\
\end{aligned} \end{equation}
Applying BC ($F(L) = 0$)
\begin{equation}\begin{aligned}
	F(L) = & c_1 (e^{\alpha_1 L} - e^{\alpha_2 L}) = 0 \\
	     = &     (e^{\alpha_1 L} - e^{\alpha_2 L}) = 0 \\
	     = &     (e^{\alpha_1 L}e^{-\alpha_2 L} - 1) = 0 \\
	       &     e^{(\alpha_1-\alpha_2) L} = 1 = e^{i2n\pi} \\
	       &     e^{(\alpha_1-\alpha_2) L} = 1 = e^{i2n\pi} \\
	       &     (\alpha_1-\alpha_2) = \frac{i2n\pi}{L} \\
	       &     (\alpha_1-\alpha_2)^2 = \left( \frac{i2n\pi}{L} \right)^2 \\
	       &     (\alpha_1-\alpha_2)^2 = - \left( \frac{2n\pi}{L} \right)^2 \\
	       &     \left(\frac{DE}{H}\right)^2 + \frac{4}{H} \gamma = - \left( \frac{2n\pi}{L} \right)^2 \\
	       &     \frac{4}{H} \gamma = - \left( \frac{2n\pi}{L} \right)^2 - \left(\frac{\kappa DE}{H}\right)^2 \\
	       &     \gamma = - \frac{H}{4} \left[ \left( \frac{2n\pi}{L} \right)^2 + \left(\frac{\kappa DE}{H}\right)^2 \right] \\
\end{aligned} \end{equation}
Returning to the $\alpha$ equation, we have
\begin{equation}\begin{aligned}
	\alpha = & i \frac{\kappa DE}{2H} \pm \frac{i}{2} \sqrt{\left(\frac{\kappa DE}{H}\right)^2 + \frac{4}{H} \gamma} \\
	\alpha = & i \frac{\kappa DE}{2H} \pm \frac{i}{2} \sqrt{\left(\frac{\kappa DE}{H}\right)^2 - \frac{4}{H} \frac{H}{4} \left[ \left( \frac{2n\pi}{L} \right)^2 + \left(\frac{\kappa DE}{H}\right)^2 \right]} \\
	\alpha = & i \frac{\kappa DE}{2H} \pm \frac{i}{2} \sqrt{-\left( \frac{2n\pi}{L} \right)^2} \\
	\alpha = & i \frac{\kappa DE}{2H} \pm \frac{-1}{2} \frac{2n\pi}{L} \\
	\alpha_1 = \bar{\alpha}_1 + i \bar{\alpha}_2 \\
	\alpha_2 = \bar{\alpha}_1 - i \bar{\alpha}_2 \\
\end{aligned} \end{equation}
So, our spatial solution becomes
\begin{equation}\begin{aligned}
	F(z) = & c_1 (e^{(\bar{\alpha}_1 + i \bar{\alpha}_2) z} - e^{(\bar{\alpha}_1 - i \bar{\alpha}_2) z}) \\
	     = & c_1 (e^{\bar{\alpha}_1 z}e^{i \bar{\alpha}_2 z} - e^{\bar{\alpha}_1 z}e^{-i \bar{\alpha}_2 z}) \\
	     = & c_1 e^{\bar{\alpha}_1 z} (e^{i \bar{\alpha}_2 z} - e^{-i \bar{\alpha}_2 z}) \\
	     = & c_1 e^{\bar{\alpha}_1 z} \sin(\bar{\alpha}_2 z) \\
\end{aligned} \end{equation}

\subsection{Temporal Solution}
The original temporal equation is
\begin{equation}\begin{aligned}
\dot{Q} = -Q \gamma_n \\
\end{aligned} \end{equation}
Assuming a solution of the form $Q = D_1 e^{-\omega t}$, we have
\begin{equation}\begin{aligned}
\omega_n = \gamma_n \\
\end{aligned} \end{equation}

\subsection{General Solution}
Our general solution is then:
\begin{equation}\begin{aligned}
	\MAC X = \MAC X_n + \sum_{n=0}^{\infty} \sum_{n=0}^{\infty} D_n e^{-\frac{H}{4} \left[ \left(\frac{DE}{H}\right)^2 + \left( \frac{2n\pi}{L} \right)^2  \right] t} e^{-\frac{\kappa DE}{2H} z} \sin\left(\frac{n\pi}{L} z \right) \\
\end{aligned} \end{equation}
Applying the initial condition, we have
\begin{equation}\begin{aligned}
	\MAC X(z,0) = \MAC X_n(z,0) + \sum_{n=0}^{\infty} \sum_{n=0}^{\infty} D_n e^{-\frac{\kappa DE}{2H} z} \sin\left(\frac{n\pi}{L} z \right) = (- \kappa EC -G) \\
\end{aligned} \end{equation}


\end{document}