\documentclass[11pt]{article}
\input{../includes.tex}

\begin{document}
\doublespacing
\MOONSTITLE
\maketitle

\section{Solving Shercliff-modified governing equations}
In this document, we attempt the solution to the decoupled equations
\begin{equation}\begin{aligned}
\DEL^2 X + A \PD_x X = - C, \qquad \text{BCs: $X = 0 $ on $\PD \Omega$} \\
\DEL^2 Y - A \PD_x Y = - D, \qquad \text{BCs: $Y = 0 $ on $\PD \Omega$} \\
\end{aligned} \end{equation}
Where constant $A$ is assumed to be positive. We assume the solution is the sum of a homogeneous equation, where $C,D$, are neglected, plus a solution with the coefficients present.
\begin{equation}\begin{aligned}
X = X_h(x,y) + X_p(y) \\
Y = Y_h(x,y) + Y_p(y) \\
\end{aligned} \end{equation}
\begin{equation}\begin{aligned}
\DEL^2 X_h + A \PD_x X_h = 0, \qquad\qquad \DEL^2 X_p = -C \\
\DEL^2 Y_h - A \PD_x Y_h = 0, \qquad\qquad \DEL^2 Y_p = -D \\
\end{aligned} \end{equation}

\section{Homogeneous solution for X}
Governing equation
\begin{equation}\begin{aligned}
\DEL^2 X_h + A \PD_x X_h = 0, \qquad\qquad X_h = X_h(x,y) \\
\end{aligned} \end{equation}
Assume the solution is separable:
\begin{equation}\begin{aligned}
X_h(x,y) = F(x)G(y) \\
\end{aligned} \end{equation}
Governing equation becomes
\begin{equation}\begin{aligned}
G F'' + FG'' + A G F' = 0 \\
 \frac{F''}{F} + \frac{G''}{G} + A \frac{F'}{F} = 0 \\
 \frac{F''}{F} + A \frac{F'}{F} = - \frac{G''}{G} = \lambda \\
\end{aligned} \end{equation}

\noindent\begin{minipage}[b]{.5\linewidth}\centering
\begin{equation}\begin{aligned}
\frac{F''}{F} + A \frac{F'}{F} = \lambda \\
F'' + A F' - F \lambda = 0 \\
F = \alpha e^{\gamma x} \\
\gamma^2 + A \gamma - \lambda = 0 \\
\gamma_{1,2} = -A \pm \frac{\sqrt{A^2 + 4\lambda}}{2} \\
F_n = \alpha_1 e^{\gamma_1 x} + \alpha_2 e^{\gamma_2 x} \\
\text{Let $\alpha_1,\alpha_2$ absorb $e^{-A}$} \\
\gamma_{1,2} = \pm \frac{\sqrt{A^2 + 4\lambda}}{2} \\
F_n = \alpha_1 e^{\gamma_1 x} + \alpha_2 e^{\gamma_2 x} \\
\end{aligned} \end{equation}
\end{minipage}
\noindent\begin{minipage}[b]{.5\linewidth}\centering
\begin{equation}\begin{aligned}
\frac{G''}{G} = - \lambda \\
G'' + G \lambda = 0 \\
G = \beta e^{\theta y} \\
\theta^2 + \lambda = 0 \\
\theta_{1,2} = \pm i \sqrt{\lambda} \\
G = \beta_1 e^{i \sqrt{\lambda} y} + \beta_2 e^{-i \sqrt{\lambda} y} \\
G'(0) = \beta_1 i \sqrt{\lambda} - \beta_2 i \sqrt{\lambda} = 0 \\
\beta_2 = \beta_1 \\
G(y) = \beta_1 (e^{ i \sqrt{\lambda} y} + e^{-i \sqrt{\lambda} y}) = 0 \\
G(b) = \beta_1 (e^{ i \sqrt{\lambda} b} + e^{-i \sqrt{\lambda} b}) = 0 \\
                e^{2i \sqrt{\lambda} b} = -1 \\
2i \sqrt{\lambda} b = 2 \pi i (n+1/2) \\
   \sqrt{\lambda} b =   \pi   (n+1/2) \\
         \lambda_n  = \left(\frac{\pi}{b} \left( n+\frac{1}{2} \right) \right)^2 \\
G(y) = 2 \beta_1 \cos(\sqrt{\lambda_n} y) \\
\end{aligned} \end{equation}
\end{minipage}
Our general solution to the homogeneous solution is then
\begin{equation}\begin{aligned}
X_h = \sum_{n=1}^{\infty} \left( {\alpha_n}_1 e^{{\gamma_n}_1 x} + {\alpha_n}_2 e^{{\gamma_n}_2 x} \right) \cos(\sqrt{\lambda_n} y) \\
\end{aligned} \end{equation}

\section{Homogeneous solution for Y}
Governing equation
\begin{equation}\begin{aligned}
\DEL^2 Y_h - A \PD_x Y_h = 0, \qquad\qquad Y_h = Y_h(x,y) \\
\end{aligned} \end{equation}
Assume the solution is separable:
\begin{equation}\begin{aligned}
Y_h(x,y) = F(x)G(y) \\
\end{aligned} \end{equation}
\begin{equation}\begin{aligned}
G F'' + FG'' - A G F' = 0 \\
 \frac{F''}{F} + \frac{G''}{G} - A \frac{F'}{F} = 0 \\
 \frac{F''}{F} - A \frac{F'}{F} = - \frac{G''}{G} = \lambda \\
\end{aligned} \end{equation}

\noindent\begin{minipage}[b]{.5\linewidth}\centering
\begin{equation}\begin{aligned}
\frac{F''}{F} - A \frac{F'}{F} = \lambda \\
F'' - A F' - F \lambda = 0 \\
F = \alpha e^{\gamma x} \\
\gamma^2 - A \gamma - \lambda = 0 \\
\gamma_{1,2} = A \pm \frac{\sqrt{A^2 + 4\lambda}}{2} \\
F_n = \alpha_1 e^{\gamma_1 x} + \alpha_2 e^{\gamma_2 x} \\
\text{Let $\alpha_1,\alpha_2$ absorb $e^{A}$} \\
\gamma_{1,2} = \pm \frac{\sqrt{A^2 + 4\lambda}}{2} \\
F_n = \alpha_1 e^{\gamma_1 x} + \alpha_2 e^{\gamma_2 x} \\
\end{aligned} \end{equation}
\end{minipage}
\noindent\begin{minipage}[b]{.5\linewidth}\centering
\begin{equation}\begin{aligned}
\frac{G''}{G} = - \lambda \\
G'' + G \lambda = 0 \\
G = \beta e^{\theta y} \\
\theta^2 + \lambda = 0 \\
\theta_{1,2} = \pm i \sqrt{\lambda} \\
G = \beta_1 e^{i \sqrt{\lambda} y} + \beta_2 e^{-i \sqrt{\lambda} y} \\
G'(0) = \beta_1 i \sqrt{\lambda} - \beta_2 i \sqrt{\lambda} = 0 \\
\beta_2 = \beta_1 \\
G(y) = \beta_1 (e^{ i \sqrt{\lambda} y} + e^{-i \sqrt{\lambda} y}) = 0 \\
G(b) = \beta_1 (e^{ i \sqrt{\lambda} b} + e^{-i \sqrt{\lambda} b}) = 0 \\
                e^{2i \sqrt{\lambda} b} = -1 \\
2i \sqrt{\lambda} b = 2 \pi i (n+1/2) \\
   \sqrt{\lambda} b =   \pi   (n+1/2) \\
\lambda_n  = \left(\frac{\pi}{b} \left( n+\frac{1}{2} \right) \right)^2 \\
G(y) = 2 \beta_1 \cos(\sqrt{\lambda_n} y) \\
\end{aligned} \end{equation}
\end{minipage}
Our general solution to the homogeneous solution is then
\begin{equation}\begin{aligned}
Y_h = \sum_{n=1}^{\infty} \left( {\alpha_n}_1 e^{\gamma_1 x} + {\alpha_n}_2 e^{\gamma_2 x} \right) \cos(\sqrt{\lambda_n} y) \\
\end{aligned} \end{equation}

\section{Homogeneous solution summary}
\begin{equation}\begin{aligned}
X_h = \sum_{n=1}^{\infty} \left( {\alpha_n}_1 e^{{\gamma_n}_1 x} + {\alpha_n}_2 e^{{\gamma_n}_2 x} \right) \cos(\sqrt{\lambda_n} y) \\
Y_h = \sum_{n=1}^{\infty} \left( {\alpha_n}_1 e^{{\gamma_n}_1 x} + {\alpha_n}_2 e^{{\gamma_n}_2 x} \right) \cos(\sqrt{\lambda_n} y) \\
\end{aligned} \end{equation}

\section{Non-homogeneous solution}
Governing equation
\begin{equation}\begin{aligned}
\DEL^2 X_p = -C, \qquad X_p = X_p(y) \\
\DEL^2 Y_p = -D, \qquad Y_p = Y_p(y) \\
\end{aligned} \end{equation}
The solution only depends on $y$:
\begin{equation}\begin{aligned}
X_p'' = -C \\
Y_p'' = -D \\
\end{aligned} \end{equation}
So integration is trivially performed. First integration yields
\begin{equation}\begin{aligned}
X_p' = -C y + c_1 \\
Y_p' = -D y + b_1 \\
\end{aligned} \end{equation}
Second integration yields
\begin{equation}\begin{aligned}
X_p = -C \frac{1}{2} y^2 + c_1 y + c_2 \\
Y_p = -D \frac{1}{2} y^2 + b_1 y + b_2 \\
\end{aligned} \end{equation}
Applying BCs, we have:
\begin{equation}\begin{aligned}
X_p(-b) = 0 = -C \frac{1}{2} b^2 - c_1 b + c_2 \\
Y_p(-b) = 0 = -D \frac{1}{2} b^2 - b_1 b + b_2 \\
X_p(b) = 0 = -C \frac{1}{2} b^2 + c_1 b + c_2 \\
Y_p(b) = 0 = -D \frac{1}{2} b^2 + b_1 b + b_2 \\
C \frac{1}{2} b^2 = c_2 \\
D \frac{1}{2} b^2 = b_2 \\
c_1 = 0 \\
b_1 = 0 \\
\end{aligned} \end{equation}
The particular solution is then
\begin{equation}\begin{aligned}
X_p = -C \frac{1}{2} y^2 + C \frac{1}{2} b^2 \\
Y_p = -D \frac{1}{2} y^2 + D \frac{1}{2} b^2 \\
\end{aligned} \end{equation}
Or
\begin{equation}\begin{aligned}
X_p = C \frac{1}{2} (b^2 - y^2) \\
Y_p = D \frac{1}{2} (b^2 - y^2) \\
\end{aligned} \end{equation}

\section{Total solution}
The total general solution is therefore:
\begin{equation}\begin{aligned}
X = C \frac{1}{2} (b^2 - y^2) + \sum_{n=1}^{\infty} \left( {\alpha_n}_1 e^{{\gamma_n}_1 x} + {\alpha_n}_2 e^{{\gamma_n}_2 x} \right) \cos(\sqrt{\lambda_n} y) \\
Y = D \frac{1}{2} (b^2 - y^2) + \sum_{n=1}^{\infty} \left( {\beta_n}_1  e^{{\gamma_n}_1 x} + {\beta_n}_2  e^{{\gamma_n}_2 x} \right) \cos(\sqrt{\lambda_n} y) \\
\end{aligned} \end{equation}
Finally, the BCs at $x=0,a$ must be applied:
Quick aside

\noindent \rule{\textwidth}{1pt}
Fourier series coefficients over the domain $[0,L]$
\begin{equation}\begin{aligned}
f(x) = \frac{A_0}{2} + \sum_{n=1}^{\infty} \left[ A_n \cos\left( \frac{n \pi x}{L} \right) + B_n \sin\left( \frac{n \pi x}{L} \right) \right] \\
\end{aligned} \end{equation}
may be solved using
\begin{equation}\begin{aligned}
A_0 = \frac{2}{L} \int_0^L f(x) dx, \qquad
A_n = \frac{2}{L} \int_0^L f(x) \cos\left( \frac{n \pi x}{L} \right) dx, \qquad
B_n = \frac{2}{L} \int_0^L f(x) \sin\left( \frac{n \pi x}{L} \right) dx
\end{aligned} \end{equation}
or over the domain $[-L,L]$:
\begin{equation}\begin{aligned}
A_0 = \frac{1}{L} \int_{-L}^L f(x) dx, \qquad
A_n = \frac{1}{L} \int_{-L}^L f(x) \cos\left( \frac{n \pi x}{L} \right) dx, \qquad
B_n = \frac{1}{L} \int_{-L}^L f(x) \sin\left( \frac{n \pi x}{L} \right) dx
\end{aligned} \end{equation}
\noindent \rule{\textwidth}{1pt}

\subsection{BC at x=-a}
Applying BC at $x=-a$ yields
\begin{equation}\begin{aligned}
\sum_{n=1}^{\infty} \left( {\alpha_n}_1 e^{-{\gamma_n}_1 a} + {\alpha_n}_2 e^{-{\gamma_n}_2 a} \right) \cos(\sqrt{\lambda_n} y) = C \frac{1}{2} (y^2-b^2) \\
\sum_{n=1}^{\infty} \left( {\beta_n}_1  e^{-{\gamma_n}_1 a} + {\beta_n}_2  e^{-{\gamma_n}_2 a} \right) \cos(\sqrt{\lambda_n} y) = D \frac{1}{2} (y^2-b^2) \\
\end{aligned} \end{equation}
These are sine series expansions with respect to $y$, whose coefficients may be found from
\begin{equation}\begin{aligned}
\left( {\alpha_n}_1 e^{-{\gamma_n}_1 a} + {\alpha_n}_2 e^{-{\gamma_n}_2 a} \right) = C I_n \\
\left( {\beta_n}_1  e^{-{\gamma_n}_1 a} + {\beta_n}_2  e^{-{\gamma_n}_2 a} \right) = D I_n \\
{\alpha_n}_0 C b^2 = I_0 \\
{\beta_n}_0  D b^2 = I_0 \\
\end{aligned} \end{equation}
Where $I_n$ is defined in the next section.

\subsection{BC at x=a}
Applying BC at $x=a$ yields
\begin{equation}\begin{aligned}
\sum_{n=1}^{\infty} \left( {\alpha_n}_1 e^{{\gamma_n}_1 a} + {\alpha_n}_2 e^{{\gamma_n}_2 a} \right) \cos(\sqrt{\lambda_n} y) = C \frac{1}{2} (y^2 - b^2) \\
\sum_{n=1}^{\infty} \left( {\beta_n}_1  e^{{\gamma_n}_1 a} + {\beta_n}_2  e^{{\gamma_n}_2 a} \right) \cos(\sqrt{\lambda_n} y) = D \frac{1}{2} (y^2 - b^2) \\
\end{aligned} \end{equation}

These are sine series expansions with respect to $y$, whose coefficients may be found from the same integral as before, so we have
\begin{equation}\begin{aligned}
\left( {\alpha_n}_1 e^{{\gamma_n}_1 a} + {\alpha_n}_2 e^{{\gamma_n}_2 a} \right) = C I_n \\
\left( {\beta_n}_1  e^{{\gamma_n}_1 a} + {\beta_n}_2  e^{{\gamma_n}_2 a} \right) = D I_n \\
\end{aligned} \end{equation}
Where $I_n$ is defined in the next section.

\section{Evaluating the integral}
The integral from the previous section is
\begin{equation}\begin{aligned}
I_0 = \frac{1}{b} \int_{-b}^{b} \frac{1}{2} (y^2 - b^2) dy \\
I_n = \frac{1}{b} \int_{-b}^{b} \frac{1}{2} (y^2 - b^2) \cos(\sqrt{\lambda_n} y) dy \\
\end{aligned} \end{equation}
The integral yields (via Wolfram alpha)
\begin{equation}\begin{aligned}
I_0 = - \frac{2}{3} b^2 \\
I_{n} = \frac{1}{b} \left( \frac{2 b \cos{ \left( b \sqrt{\lambda_n} \right) }}{\lambda_n}-\frac{2 \sin{ \left( b \sqrt{\lambda_n} \right) }}{\lambda_n^{3/2}} \right) \\
\end{aligned} \end{equation}

\section{Combining BC equations}
Now we can combine the equations from each BC:


\begin{equation}\begin{aligned}
{\alpha_n}_0 C b^2 = - \frac{2}{3} b^2, \qquad {\alpha_n}_0 = -\frac{2}{3 C} \\
{\beta_n}_0  D b^2 = - \frac{2}{3} b^2, \qquad {\beta_n}_0  = -\frac{2}{3 D} \\
\left( {\alpha_n}_1 e^{-{\gamma_n}_1 a} + {\alpha_n}_2 e^{-{\gamma_n}_2 a} \right) = C I_n \\
\left( {\alpha_n}_1 e^{ {\gamma_n}_1 a} + {\alpha_n}_2 e^{ {\gamma_n}_2 a} \right) = C I_n \\
\left( {\beta_n}_1  e^{-{\gamma_n}_1 a} + {\beta_n}_2  e^{-{\gamma_n}_2 a} \right) = D I_n \\
\left( {\beta_n}_1  e^{ {\gamma_n}_1 a} + {\beta_n}_2  e^{ {\gamma_n}_2 a} \right) = D I_n \\
\end{aligned} \end{equation}
We have 4 equations and 4 unknowns

\section{Simplified equation form}
Both sets of equations are in the form
\begin{equation}\begin{aligned}
A_1 E_1 + A_2 E_2 = H \\
A_1 F_1 + A_2 F_2 = H \\
\end{aligned} \end{equation}
The solution to this system is
\begin{equation}\begin{aligned}
A_1 = \frac{H}{\theta} (E_2 - F_2) \\
A_2 = \frac{H}{\theta} (F_1 - E_1) \\
\theta = F_1 E_2 - F_2 E_1 \\
\end{aligned} \end{equation}

\section{Combining BC equations (continued)}
Solving the BC system yields
\begin{equation}\begin{aligned}
{\alpha_n}_0 = -\frac{2}{3 C} \\
{\beta_n}_0  = -\frac{2}{3 D} \\
\theta = e^{ {\gamma_n}_1 a} e^{-{\gamma_n}_2 a} - e^{ {\gamma_n}_2 a} e^{-{\gamma_n}_1 a} \\
{\alpha_n}_1 = \frac{H}{\theta} (E_2 - F_2) = \frac{C I_n}{\theta} (e^{-{\gamma_n}_2 a} - e^{ {\gamma_n}_2 a}) \\
{\alpha_n}_2 = \frac{H}{\theta} (F_1 - E_1) = \frac{C I_n}{\theta} (e^{ {\gamma_n}_1 a} - e^{-{\gamma_n}_1 a}) \\
{\beta_n}_1  = \frac{H}{\theta} (E_2 - F_2) = \frac{D I_n}{\theta} (e^{-{\gamma_n}_2 a} - e^{ {\gamma_n}_2 a}) \\
{\beta_n}_2  = \frac{H}{\theta} (F_1 - E_1) = \frac{D I_n}{\theta} (e^{ {\gamma_n}_1 a} - e^{-{\gamma_n}_1 a}) \\
\end{aligned} \end{equation}

\section{Returning to our total solution}
Finally, we have
\begin{equation}\begin{aligned}
\lambda_n  = \left(\frac{\pi}{b} \left( n+\frac{1}{2} \right) \right)^2 \\
{\gamma_n}_{1,2} = \pm \frac{\sqrt{A^2 + 4 \lambda_n}}{2} \\
I_{n} = \frac{1}{b} \left( \frac{2 b \cos{ \left( b \sqrt{\lambda_n} \right) }}{\lambda_n}-\frac{2 \sin{ \left( b \sqrt{\lambda_n} \right) }}{\lambda_n^{3/2}} \right) \\
{\alpha_n}_0 = -\frac{2}{3 C} \\
{\beta_n}_0  = -\frac{2}{3 D} \\
\theta = e^{ {\gamma_n}_1 a} e^{-{\gamma_n}_2 a} - e^{ {\gamma_n}_2 a} e^{-{\gamma_n}_1 a} \\
{\alpha_n}_1 = \frac{C I_n}{\theta} (e^{-{\gamma_n}_2 a} - e^{ {\gamma_n}_2 a}) \\
{\alpha_n}_2 = \frac{C I_n}{\theta} (e^{ {\gamma_n}_1 a} - e^{-{\gamma_n}_1 a}) \\
{\beta_n}_1  = \frac{D I_n}{\theta} (e^{-{\gamma_n}_2 a} - e^{ {\gamma_n}_2 a}) \\
{\beta_n}_2  = \frac{D I_n}{\theta} (e^{ {\gamma_n}_1 a} - e^{-{\gamma_n}_1 a}) \\
% X = C \frac{1}{2} (b^2 - y^2) + \sum_{n=1}^{\infty} \left( {\alpha_n}_1 e^{{\gamma_n}_1 x} + {\alpha_n}_2 e^{{\gamma_n}_2 x} \right) \cos(\sqrt{\lambda_n} y) \\
% Y = D \frac{1}{2} (b^2 - y^2) + \sum_{n=1}^{\infty} \left( {\beta_n}_1  e^{{\gamma_n}_1 x} + {\beta_n}_2  e^{{\gamma_n}_2 x} \right) \cos(\sqrt{\lambda_n} y) \\
X = -\frac{b^2}{3} - C \frac{1}{2} y^2 + \sum_{n=1}^{\infty} \left( {\alpha_n}_1 e^{{\gamma_n}_1 x} + {\alpha_n}_2 e^{{\gamma_n}_2 x} \right) \cos(\sqrt{\lambda_n} y) \\
Y = -\frac{b^2}{3} - D \frac{1}{2} y^2 + \sum_{n=1}^{\infty} \left( {\beta_n}_1  e^{{\gamma_n}_1 x} + {\beta_n}_2  e^{{\gamma_n}_2 x} \right) \cos(\sqrt{\lambda_n} y) \\
\end{aligned} \end{equation}

Solutions are reconstructed using:
\begin{equation}\begin{aligned}
w   =                 \frac{1}{2} (X + Y)\\
B_z = \frac{Re_m}{Ha} \frac{1}{2} (X - Y)\\
\end{aligned} \end{equation}


\end{document}