\documentclass[11pt]{article}
\newcommand{\PSCHAIN}{..}
\input{../prepend_PS_chain}
\newcommand{\rootdir}{\PSCHAIN}
\input{\PSCHAIN/includes/includes}


\begin{document}
\doublespacing
\MOONSTITLE
\maketitle

\section{LSA - removing base equations of SK flow}

The LSA governing equations (derived elsewhere) are
\begin{equation}\begin{aligned}
\PD_t v' = -\frac{1}{\rho}\PD_y p' + \nu (\PD_{yy} v'+\PD_{zz} v') - \frac{1}{\rho \M} \left( B_x^0 \PD_y B_x^1 + B_x^0 \PD_y B_x^{1'} \right) \\
\PD_t w' = -\frac{1}{\rho}\PD_z p' + \nu (\PD_{yy} w'+\PD_{zz} w') - \frac{1}{\rho \M} \left( B_x^0 \PD_z B_x^1 + B_x^0 \PD_z B_x^{1'} \right) \\
\PD_t (B_x^{0}+B_x^{1}+B_x^{1'}) = \frac{1}{\sigma \M} (\PD_{yy} (B_x^{1}+B_x^{1'})+\PD_{zz} (B_x^{1}+B_x^{1'})) \\
\PD_y v' + \PD_z w' = 0  \\
\end{aligned} \end{equation}

First, let's neglect dynamic viscosity
\begin{equation}\begin{aligned}
\PD_t v' = -\frac{1}{\rho}\PD_y p' - \frac{1}{\rho \M} \left( B_x^0 \PD_y B_x^1 + B_x^0 \PD_y B_x^{1'} \right) \\
\PD_t w' = -\frac{1}{\rho}\PD_z p' - \frac{1}{\rho \M} \left( B_x^0 \PD_z B_x^1 + B_x^0 \PD_z B_x^{1'} \right) \\
\PD_t (B_x^{0}+B_x^{1}+B_x^{1'}) = \frac{1}{\sigma \M} (\PD_{yy} (B_x^{1}+B_x^{1'})+\PD_{zz} (B_x^{1}+B_x^{1'})) \\
\PD_y v' + \PD_z w' = 0  \\
\end{aligned} \end{equation}
Now, let's assume a steady equilibrium $B_x^1$ and move the equilibrium $B_x^1$ terms into pressure. The new pressure will be denoted as $P$. Also, since $\PD_t B_x^0$ is the only forcing term, let's denote this as $\theta$.
\begin{equation}\begin{aligned}
\PD_t v' = -\frac{1}{\rho}\PD_y P' - \frac{1}{\rho \M} B_x^0 \PD_y B_x^{1'} \\
\PD_t w' = -\frac{1}{\rho}\PD_z P' - \frac{1}{\rho \M} B_x^0 \PD_z B_x^{1'} \\
\theta + \PD_t B_x^{1'} = \frac{1}{\sigma \M} (\PD_{yy} (B_x^{1}+B_x^{1'})+\PD_{zz} (B_x^{1}+B_x^{1'})) \\
\PD_y v' + \PD_z w' = 0  \\
\end{aligned} \end{equation}
The "base" $B_x^1$ is zero, so we have
\begin{equation}\begin{aligned}
\PD_t v' = -\frac{1}{\rho}\PD_y P' - \frac{1}{\rho \M} B_x^0 \PD_y B_x^{1'} \\
\PD_t w' = -\frac{1}{\rho}\PD_z P' - \frac{1}{\rho \M} B_x^0 \PD_z B_x^{1'} \\
\theta + \PD_t B_x^{1'} = \frac{1}{\sigma \M} (\PD_{yy} B_x^{1'}+\PD_{zz} B_x^{1'}) \\
\PD_y v' + \PD_z w' = 0  \\
\end{aligned} \end{equation}
For convenience, let's remove the primes
\begin{equation}\begin{aligned}
\PD_t v = -\frac{1}{\rho}\PD_y P - \frac{1}{\rho \M} B_x^0 \PD_y B_x^{1} \\
\PD_t w = -\frac{1}{\rho}\PD_z P - \frac{1}{\rho \M} B_x^0 \PD_z B_x^{1} \\
\theta + \PD_t B_x^{1} = \frac{1}{\sigma \M} (\PD_{yy} B_x^{1}+\PD_{zz} B_x^{1}) \\
\PD_y v + \PD_z w = 0  \\
\end{aligned} \end{equation}


\end{document}