\documentclass[11pt]{article}
\input{../includes.tex}

\begin{document}
\doublespacing
\MOONSTITLE
\maketitle

\section{Decoupling of 1D plasma-disruption governing equations}
In this document, decouple the 1D plasma disruption governing equations
\begin{equation}\begin{aligned}
u''   = - \frac{1}{\rho \nu \M} B_z^0 B_x' \\
B_x'' = \sigma \M (\PD_t B_x^0 - B_z^0 u') \\
\end{aligned} \end{equation}
Let
\begin{equation}\begin{aligned}
A = \frac{1}{\rho \nu \M} B_z^0, \qquad
C = \sigma \M \PD_t B_x^0, \qquad
D = \sigma \M B_z^0
\end{aligned} \end{equation}
\begin{equation}\begin{aligned}
u''   = - A B_x' \\
B_x'' = C - D u' \\
\end{aligned} \end{equation}

\section{Variable seperation transformation}
We may apply the transformation
\begin{equation}\begin{aligned}
X = u + F B_x \\
Y = u - F B_x \\
\end{aligned} \end{equation}

\subsection{Transformation for X}
We have
\begin{equation}\begin{aligned}
(X - F B_x)''   = - A B_x' \\
B_x'' = C - D (X - F B_x)' \\
\end{aligned} \end{equation}
Distributing
\begin{equation}\begin{aligned}
X'' - F B_x''   = - A B_x' \\
B_x'' = C - D X' + D F B_x' \\
\end{aligned} \end{equation}
Combining with factor $E$ for second equation
\begin{equation}\begin{aligned}
X'' - F B_x'' + FB_x''   = - A B_x' + E(C - D X' + D F B_x') \\
\end{aligned} \end{equation}
To ensure $B_x$ dissappears, we must enforce
\begin{equation}\begin{aligned}
-F + E = 0, \qquad E = F \\
-A + FDE = 0,\qquad E^2D = A, \qquad E = F = \sqrt{\frac{A}{D}}\\
\end{aligned} \end{equation}
So we have
\begin{equation}\begin{aligned}
X'' - F B_x'' + FB_x''   = - A B_x' + E(C - D X' + D F B_x') \\
X'' = - A B_x' + FC - FD X' + E^2 D B_x' \\
X'' = FC - FD X' + (E^2 D B_x' - A B_x') \\
X'' = FC - FD X' + \left(\frac{A}{D} D B_x' - A B_x' \right) \\
X'' = FC - FD X' \\
\end{aligned} \end{equation}
\subsection{Transformation for Y}
Reminder
\begin{equation}\begin{aligned}
u''   = - A B_x' \\
B_x'' = C - D u' \\
\end{aligned} \end{equation}
We have
\begin{equation}\begin{aligned}
(Y + F B_x)''   = - A B_x' \\
B_x'' = C - D (Y + F B_x)' \\
\end{aligned} \end{equation}
Distributing
\begin{equation}\begin{aligned}
Y'' + F B_x''   = - A B_x' \\
B_x'' = C - D Y' - D F B_x' \\
\end{aligned} \end{equation}
Combining with factor $-E$ for second equation yields
\begin{equation}\begin{aligned}
Y'' + F B_x'' - FB_x''   = - A B_x' - E(C - D Y' - D F B_x') \\
Y'' = - A B_x' - FC + E D Y' + E D F B_x' \\
Y'' = - FC + E D Y' + (E D F B_x' - A B_x') \\
Y'' = - FC + E D Y' + \left(\frac{A}{D} D B_x' - A B_x' \right) \\
Y'' = - FC + F D Y' \\
\end{aligned} \end{equation}
\section{Transformation summary}
Our decoupled equations are
\begin{equation}\begin{aligned}
X'' + F D X' =   FC \\
Y'' - F D Y' = - FC \\
\end{aligned} \end{equation}
Where
\begin{equation}\begin{aligned}
A = \frac{1}{\rho \nu \M} B_z^0, \qquad
C = \sigma \M \PD_t B_x^0, \qquad
D = \sigma \M B_z^0, \qquad
F = \sqrt{\frac{A}{D}} \\
\end{aligned} \end{equation}
With transformations
\begin{equation}\begin{aligned}
X = u + F B_x \\
Y = u - F B_x \\
\end{aligned} \end{equation}
And inverse transformations
\begin{equation}\begin{aligned}
u   = \frac{1}{2} \left( X + Y \right) \\
B_x = \frac{1}{2E} \left( X - Y \right) \\
\end{aligned} \end{equation}
\begin{equation}\begin{aligned}
A = \frac{1}{\rho \nu \M} B_z^0, \qquad
C = \sigma \M \PD_t B_x^0, \qquad
D = \sigma \M B_z^0, \qquad
F = \sqrt{\frac{A}{D}} \\
\end{aligned} \end{equation}


\end{document}