\documentclass[11pt]{article}
\newcommand{\PSCHAIN}{..}
\input{../prepend_PS_chain}
\newcommand{\rootdir}{\PSCHAIN}
\input{\PSCHAIN/includes/includes}

\newcommand{\HALF}{\frac{1}{2}}

\begin{document}
\doublespacing
\MOONSTITLE
\maketitle

\section{Transformation}
The Hartmann flow governing equations are:

\begin{equation}\begin{aligned}
\frac{1}{\rho}\PD_x p = \nu \PD_{yy} u + \frac{1}{\rho \M} B_y^0 \PD_y B_x \\
\PD_{yy} B_x = - \sigma \M B_y^0 \PD_y u \\
\end{aligned} \end{equation}

Or, since $y$ is the only variable, we have
\begin{equation}\begin{aligned}
\frac{1}{\rho}\PD_x p = \nu u'' + \frac{1}{\rho \M} B_y^0 B_x' \\
B_x'' = - \sigma \M B_y^0 u' \\
\end{aligned} \end{equation}

Introducing the variable transformation
\begin{equation}\begin{aligned}
X = u + C B_x \\
Y = u - C B_x \\
\end{aligned} \end{equation}
Let's look at each transformation
\subsection{X transformation}
We have
\begin{equation}\begin{aligned}
\frac{1}{\rho}\PD_x p = \nu (X''-C B_x'') + \frac{1}{\rho \M} B_y^0 B_x' \\
B_x'' = - \sigma \M B_y^0 (X' - C B_x') \\
\end{aligned} \end{equation}
Therefore
\begin{equation}\begin{aligned}
\frac{1}{\rho}\PD_x p = \nu (X''-C (- \sigma \M B_y^0 (X' - C B_x'))) + \frac{1}{\rho \M} B_y^0 B_x' \\
\frac{1}{\rho}\PD_x p = \nu (X''+C \sigma \M B_y^0 (X' - C B_x')) + \frac{1}{\rho \M} B_y^0 B_x' \\
\frac{1}{\rho}\PD_x p = \nu (X''+ C \sigma \M B_y^0 X' - C^2 \sigma \M B_y^0 B_x') + \frac{1}{\rho \M} B_y^0 B_x' \\
\frac{1}{\rho}\PD_x p = \nu X''+ C \nu \sigma \M B_y^0 X' - C^2 \nu \sigma \M B_y^0 B_x' + \frac{1}{\rho \M} B_y^0 B_x' \\
\end{aligned} \end{equation}
We need $B_x'$ to dropout, therefore we need $C$ such that
\begin{equation}\begin{aligned}
- C^2 \nu \sigma \M B_y^0 B_x' + \frac{1}{\rho \M} B_y^0 B_x' = 0 \\
C^2 \nu \sigma \M = \frac{1}{\rho \M} \\
C^2 = \frac{1}{ \mu \sigma \M^2} \\
C = \frac{1}{\M \sqrt{\mu \sigma}} \\
\end{aligned} \end{equation}
Our governing equation is then
\begin{equation}\begin{aligned}
\nu X''+ \frac{1}{\M \sqrt{\mu \sigma}} \nu \sigma \M B_y^0 X' = \frac{1}{\rho}\PD_x p \\
\nu X''+ \frac{1}{\sqrt{\rho \nu \sigma}} \nu \sigma B_y^0 X' = \frac{1}{\rho}\PD_x p \\
\nu X''+ \frac{\sqrt{\nu \sigma}}{\sqrt{\rho}} B_y^0 X' = \frac{1}{\rho}\PD_x p \\
\mu X''+ \sqrt{\mu \sigma} B_y^0 X' = \PD_x p\\
\end{aligned} \end{equation}

\subsection{Y transformation}
Now the $Y$ transformation:
\begin{equation}\begin{aligned}
\frac{1}{\rho}\PD_x p = \nu (Y'' + C B_x'') + \frac{1}{\rho \M} B_y^0 B_x' \\
B_x'' = - \sigma \M B_y^0 (Y' + C B_x') \\
\end{aligned} \end{equation}
Therefore
\begin{equation}\begin{aligned}
\frac{1}{\rho}\PD_x p = \nu (Y'' + C (- \sigma \M B_y^0 (Y' + C B_x'))) + \frac{1}{\rho \M} B_y^0 B_x' \\
\frac{1}{\rho}\PD_x p = \nu Y'' + \nu C (- \sigma \M B_y^0 (Y' + C B_x')) + \frac{1}{\rho \M} B_y^0 B_x' \\
\frac{1}{\rho}\PD_x p = \nu Y'' - C \nu \sigma \M B_y^0 (Y' + C B_x') + \frac{1}{\rho \M} B_y^0 B_x' \\
\frac{1}{\rho}\PD_x p = \nu Y'' - C \nu \sigma \M B_y^0 Y' - C^2 \nu \sigma \M B_y^0 B_x' + \frac{1}{\rho \M} B_y^0 B_x' \\
\end{aligned} \end{equation}
Again, we need $B_x'$ to dropout, therefore we need $C$ such that
\begin{equation}\begin{aligned}
- C^2 \nu \sigma \M B_y^0 B_x' + \frac{1}{\rho \M} B_y^0 B_x' = 0 \\
- C^2 \nu \sigma \M + \frac{1}{\rho \M} = 0 \\
C^2 = \frac{1}{\mu \sigma \M^2} = 0 \\
C = \frac{1}{\M \sqrt{\mu \sigma}} \\
\end{aligned} \end{equation}
Same as before. Therefore, our equation is:
\begin{equation}\begin{aligned}
\nu Y'' - \frac{1}{\M \sqrt{\mu \sigma}} \nu \sigma \M B_y^0 Y' = \frac{1}{\rho}\PD_x p\\
\nu Y'' - \frac{1}{\sqrt{\mu \sigma}} \nu \sigma B_y^0 Y' = \frac{1}{\rho}\PD_x p\\
\nu Y'' - \frac{\sqrt{\nu \sigma}}{\sqrt{\rho}} B_y^0 Y' = \frac{1}{\rho}\PD_x p\\
\mu Y'' - \sqrt{\mu \sigma} B_y^0 Y' = \PD_x p\\
\end{aligned} \end{equation}

\subsection{Transformation summary}
Our decoupled, transformed governing equations are then:
\begin{equation}\begin{aligned}
C = \frac{1}{\M \sqrt{\mu \sigma}} \\
X = u + C B_x \\
Y = u - C B_x \\
\mu X'' + \sqrt{\mu \sigma} B_y^0 X' = \PD_x p\\
\mu Y'' - \sqrt{\mu \sigma} B_y^0 Y' = \PD_x p\\
\end{aligned} \end{equation}
Writing this in a more compact form, we have
\begin{equation}\begin{aligned}
C = \frac{1}{\M \sqrt{\mu \sigma}} \\
D = B_y^0 \sqrt{\frac{\sigma}{\mu}} \\
F = \frac{1}{\mu} \PD_x p \\
X = u + C B_x \\
Y = u - C B_x \\
X'' + D X' = F \\
Y'' - D Y' = F \\
\end{aligned} \end{equation}

\end{document}