\documentclass[11pt]{article}
% \documentclass[11pt,landscape]{article}
\newcommand{\PSCHAIN}{..}
\input{../prepend_PS_chain}
\newcommand{\rootdir}{\PSCHAIN}
\input{\PSCHAIN/includes/includes}
% \input{\PSCHAIN/includes/zero_margins}

\newcommand{\ABA}{\bar{\alpha}_1}
\newcommand{\ABB}{\bar{\alpha}_2}

\begin{document}
\doublespacing
\MOONSTITLE
\maketitle

\section{Solving for the Undetermined Coefficients}
Our decoupled equations are
\begin{equation}\begin{aligned}
\PD_t X - H X'' - DE X'  = (- EC -G)\\
\PD_t Y - H Y'' + DE Y'  = (+ EC -G)\\
\end{aligned} \end{equation}
With transformations
\begin{equation}\begin{aligned}
X = u + E B_x \\
Y = u - E B_x \\
E = \sqrt{\frac{A}{D}} \\
\end{aligned} \end{equation}
And inverse transformations
\begin{equation}\begin{aligned}
u   = \frac{1}{2} \left( X + Y \right) \\
B_x = \frac{1}{2E} \left( X - Y \right) \\
E = \sqrt{\frac{A}{D}} = \sqrt{\frac{1}{\rho \M}} \\
\end{aligned} \end{equation}
\begin{equation}\begin{aligned}
G = \frac{1}{\rho}\PD_x p, \qquad
H = K = \nu = \frac{1}{\sigma \M}, \qquad
A = \frac{1}{\rho \M} B_z^0, \qquad
C = \PD_t B_x^0, \qquad
D = B_z^0.
\end{aligned} \end{equation}

\section{Solution generalization}
First, let's introduce a variable so that we can solve both systems simultaneously. Let $\kappa = 1$ for the $X$ equation, and $\kappa = -1$ for the $Y$ equation.
\begin{equation}\begin{aligned}
	\PD_t \MAC X - H \MAC X'' - DE \kappa \MAC X'  = (- \kappa EC -G) \\
\end{aligned} \end{equation}
\section{Solution procedure}
First, let's decompose the solution into homogeneous and non-homogeneous:
\begin{equation}\begin{aligned}
	\MAC X = \MAC X_h + \MAC X_n, \\
\end{aligned} \end{equation}
where the homogeneous solution satisfies
\begin{equation}\begin{aligned}
	\PD_t \MAC X_h - H \MAC X_h'' - DE \kappa \MAC X_h'  = 0 \\
\end{aligned} \end{equation}
Assuming the homogeneous solution is separable ($\MAC X_h(z,t) = F(z)Q(t)$), we have
\begin{equation}\begin{aligned}
	F\dot{Q} - HQF'' - \kappa DEQF' = 0 \\
\end{aligned} \end{equation}
Dividing by $FQ$ yields
\begin{equation}\begin{aligned}
	\frac{\dot{Q}}{Q} = H \frac{F''}{F} + \kappa DE \frac{F'}{F} = \text{constant} = -\gamma \\
\end{aligned} \end{equation}
\subsection{Spatial solution}
Let's solve the RHS equation:
\begin{equation}\begin{aligned}
	H F'' + \kappa DE F' = -F \gamma \\
	F'' + \frac{\kappa DE}{H} F' = -\frac{F}{H} \gamma \\
\end{aligned} \end{equation}
Let's assume $F(z) = e^{\alpha z}$, to get
\begin{equation}\begin{aligned}
	H F'' + \kappa DE F' = - F \gamma \\
	\alpha^2 + \frac{\kappa DE}{H} \alpha = - \frac{1}{H} \gamma \\
	\alpha^2 + \frac{\kappa DE}{H} \alpha + \frac{1}{H} \gamma = 0  \\
	\alpha = -\frac{\kappa DE}{2H} \pm \frac{1}{2} \sqrt{\left(\frac{\kappa DE}{H}\right)^2 - \frac{4}{H} \gamma} \\
	\alpha = -\frac{\kappa DE}{2H} \pm \frac{1}{2} \sqrt{\left(\frac{DE}{H}\right)^2 - \frac{4}{H} \gamma} \\
\end{aligned} \end{equation}

From this, we may write
\begin{equation}\begin{aligned}
	\alpha_1 + \alpha_2 = -\frac{\kappa DE}{H} \\
	\alpha_1 - \alpha_2 = \sqrt{\left(\frac{DE}{H}\right)^2 - \frac{4}{H} \gamma} \\
\end{aligned} \end{equation}

So, we have
\begin{equation}\begin{aligned}
	F(z) = c_1 e^{\alpha_1 z} + c_2 e^{\alpha_2 z} \\
\end{aligned} \end{equation}
Applying BC ($F(0) = 0$)
\begin{equation}\begin{aligned}
	F(0) = & c_1 + c_2 = 0 \\
	     = & c_2 =-c_1  \\
\end{aligned} \end{equation}
Yields
\begin{equation}\begin{aligned}
	F(z) = c_1 (e^{\alpha_1 z} - e^{\alpha_2 z}) \\
\end{aligned} \end{equation}
Applying BC ($F(L) = 0$)
\begin{equation}\begin{aligned}
	F(L) = & c_1 (e^{\alpha_1 L} - e^{\alpha_2 L}) = 0 \\
	     = &     (e^{\alpha_1 L} - e^{\alpha_2 L}) = 0 \\
	     = &     (e^{\alpha_1 L}e^{-\alpha_2 L} - 1) = 0 \\
	       &     e^{(\alpha_1-\alpha_2) L} = 1 = e^{i2n\pi} \\
	       &     e^{(\alpha_1-\alpha_2) L} = 1 = e^{i2n\pi} \\
	       &     (\alpha_1-\alpha_2) = \frac{i2n\pi}{L} \\
	       &     \left(\frac{\kappa DE}{H}\right)^2 - \frac{4}{H} \gamma = \left( \frac{i2n\pi}{L} \right)^2 \\
	       &     \frac{4}{H} \gamma = \left(\frac{\kappa DE}{H}\right)^2 - \left( \frac{i2n\pi}{L} \right)^2 \\
	       &     \gamma = \frac{H}{4} \left[ \left(\frac{\kappa DE}{H}\right)^2 - \left( \frac{i2n\pi}{L} \right)^2  \right]\\
	       &     \gamma = \frac{H}{4} \left[ \left(\frac{DE}{H}\right)^2 + \left( \frac{2n\pi}{L} \right)^2  \right]\\
\end{aligned} \end{equation}
Returning to the $\alpha$ equation, we have
\begin{equation}\begin{aligned}
	\alpha = & -\frac{\kappa DE}{2H} \pm \frac{1}{2} \sqrt{\left(\frac{DE}{H}\right)^2 - \frac{4}{H} \frac{H}{4} \left[ \left(\frac{DE}{H}\right)^2 + \left( \frac{2n\pi}{L} \right)^2  \right]} \\
	       = & -\frac{\kappa DE}{2H} \pm i \frac{n\pi}{L} \\
	\alpha_1 = \ABA + i \ABB \\
	\alpha_2 = \ABA - i \ABB \\
\end{aligned} \end{equation}
So, our spatial solution becomes
\begin{equation}\begin{aligned}
	F(z) = & c_1 (e^{(\ABA + i \ABB) z} - e^{(\ABA - i \ABB) z}) \\
	     = & c_1 (e^{\ABA z}e^{i \ABB z} - e^{\ABA z}e^{-i \ABB z}) \\
	     = & c_1 e^{\ABA z} (e^{i \ABB z} - e^{-i \ABB z}) \\
	     = & c_1 e^{\ABA z} \sin(\ABB z) \\
\end{aligned} \end{equation}

\subsection{Temporal Solution}
The original temporal equation is
\begin{equation}\begin{aligned}
\dot{Q} = -Q \gamma_n \\
\end{aligned} \end{equation}
Assuming a solution of the form $Q = D_1 e^{-\omega t}$, we have
\begin{equation}\begin{aligned}
\omega_n = \gamma_n \\
\end{aligned} \end{equation}

\subsection{General Solution}
Our general solution is then:
\begin{equation}\begin{aligned}
	\MAC X = \MAC X_n + \sum_{n=0}^{\infty} D_n e^{-\frac{H}{4} \left[ \left(\frac{DE}{H}\right)^2 + \left( \frac{2n\pi}{L} \right)^2  \right] t} e^{-\frac{\kappa DE}{2H} z} \sin\left(\frac{n\pi}{L} z \right) \\
\end{aligned} \end{equation}
Or, more compactly
\begin{equation}\begin{aligned}
	\MAC X = \MAC X_n + \sum_{n=0}^{\infty} D_n e^{-\gamma_n t} e^{\ABA z} \sin(\ABB z) \\
	\gamma_n = \frac{H}{4} \left[ \left(\frac{DE}{H}\right)^2 + \left( \frac{2n\pi}{L} \right)^2  \right] \\
	\ABA = -\frac{\kappa DE}{2H} \\
	\ABB = \frac{n\pi}{L} \\
\end{aligned} \end{equation}

To apply the initial condition, plug $X$ into the governing equations, and solve for the coefficients w.r.t. the non-homogeneous source term at $t=0$:

\begin{equation}\begin{aligned}
	\MAC X = \MAC X_n + \sum_{n=0}^{\infty} D_n e^{\gamma_n t} e^{\ABA z} \sin (\ABB z) \\
	\dot{\MAC X} = \dot{\MAC X_n} - \sum_{n=0}^{\infty} D_n \gamma_n e^{\ABA z} \sin(\ABB z) \\
	\MAC X' = \MAC X_n'   + \sum_{n=0}^{\infty} D_n ( \ABA e^{\ABA z} \sin (\ABB z) + e^{\ABA z} \ABB \cos (\ABB z) ) \\
	\MAC X' = \MAC X_n'   + \sum_{n=0}^{\infty} D_n e^{\ABA z} ( \ABA \sin (\ABB z) + \ABB \cos (\ABB z) ) \\
	\MAC X''= \MAC X_n''  + \sum_{n=0}^{\infty} D_n (e^{\ABA z} ( \ABA \ABB \cos (\ABB z) - \ABB \ABB \cos (\ABB z) ) +\ABA e^{\ABA z} ( \ABA \sin (\ABB z) + \ABB \cos (\ABB z) )) \\
	\MAC X''= \MAC X_n''  + \sum_{n=0}^{\infty} D_n e^{\ABA z} \left[ (2 \ABA \ABB - \ABB \ABB) \cos (\ABB z) + \ABA \ABA \sin (\ABB z) \right] \\
\end{aligned} \end{equation}
The governing equations are:
\begin{equation}\begin{aligned}
	\PD_t \MAC X - H \MAC X'' - DE \kappa \MAC X'  = (- \kappa EC -G) \\
\end{aligned} \end{equation}
\subsection{With homogeneous part}
So, we have (at $t=0$)
\begin{equation}\begin{aligned}
	\left( \dot{\MAC X_n} - \sum_{n=0}^{\infty} D_n \gamma_n e^{\ABA z} \sin(\ABB z) \right) \\
	 - H \left( \MAC X_n''  + \sum_{n=0}^{\infty} D_n e^{\ABA z} \left[ (2 \ABA \ABB - \ABB \ABB) \cos (\ABB z) + \ABA \ABA \sin (\ABB z) \right] \right) \\
	 - DE \kappa \left( \MAC X_n'   + \sum_{n=0}^{\infty} D_n e^{\ABA z} ( \ABA \sin (\ABB z) + \ABB \cos (\ABB z) ) \right) \\
	  = \\
	  (- \kappa EC -G) \\
\end{aligned} \end{equation}

\subsection{Try removing non-homogeneous part}
So, we have (at $t=0$)
\begin{equation}\begin{aligned}
	\left( - \sum_{n=0}^{\infty} D_n \gamma_n e^{\ABA z} \sin(\ABB z) \right) \\
	 - H \left( \sum_{n=0}^{\infty} D_n e^{\ABA z} \left[ (2 \ABA \ABB - \ABB \ABB) \cos (\ABB z) + \ABA \ABA \sin (\ABB z) \right] \right) \\
	 - DE \kappa \left( \sum_{n=0}^{\infty} D_n e^{\ABA z} ( \ABA \sin (\ABB z) + \ABB \cos (\ABB z) ) \right) \\
	  = \\
	  (- \kappa EC -G) \\
\end{aligned} \end{equation}
Removing negative signs yields
\begin{equation}\begin{aligned}
	\left( \sum_{n=0}^{\infty} D_n \gamma_n e^{\ABA z} \sin(\ABB z) \right) \\
	 + H \left( \sum_{n=0}^{\infty} D_n e^{\ABA z} \left[ (2 \ABA \ABB - \ABB \ABB) \cos (\ABB z) + \ABA \ABA \sin (\ABB z) \right] \right) \\
	 + DE \kappa \left( \sum_{n=0}^{\infty} D_n e^{\ABA z} ( \ABA \sin (\ABB z) + \ABB \cos (\ABB z) ) \right) \\
	  = \\
	  (\kappa EC +G) \\
\end{aligned} \end{equation}
Factoring and collecting sin and cosine terms:
\begin{equation}\begin{aligned}
	 \sum_{n=0}^{\infty} D_n e^{\ABA z} \left[ (\gamma_n + H \ABA \ABA + DE \kappa \ABA) \sin(\ABB z) + (H(2 \ABA \ABB - \ABB \ABB) + DE\kappa \ABB ) \cos (\ABB z) \right] \\ = (\kappa EC + G) \\
\end{aligned} \end{equation}


\end{document}