\documentclass[11pt]{article}
% \documentclass[3p,twocolumn,10pt]{elsarticle}
\usepackage{graphicx}    % needed for including graphics e.g. EPS, PS
\usepackage{epstopdf}
\usepackage{amsmath}
\usepackage{amssymb}
\usepackage{hyperref}
\usepackage{xspace}
\usepackage{mathtools}
\usepackage{tikz}
\usepackage{epsfig}
\usepackage{float}
%\usepackage{natbib}
\usepackage{subfigure}
\usepackage{setspace}
\usepackage{tabularx,ragged2e,booktabs,caption}

\usepackage{xcolor}
\usepackage{xspace}
\usepackage{longtable}
\usepackage{mathtools}
\usepackage{natbib}
\usepackage{setspace}
\usepackage{ragged2e}
\usepackage{etoolbox}
\usepackage{geometry}

\input{../../../../useful_commands.tex}

\newcommand{\volume}{\mathop{\ooalign{\hfil$V$\hfil\cr\kern0.08em--\hfil\cr}}\nolimits}
\newcommand{\figWidth}{0.45\textwidth}
\newcommand{\figSuffix}{_png.png}
\newcommand{\pushright}[1]{\ifmeasuring@#1\else\omit\hfill$\displaystyle#1$\fi\ignorespaces}
\newcommand{\hfillMath}{\hskip \textwidth minus \textwidth}

\setlength{\oddsidemargin}{0.1in}
\setlength{\textwidth}{7.25in}

\setlength{\topmargin}{-1in}     %\topmargin: gap above header
\setlength{\headheight}{0in}     %\headheight: height of header
\setlength{\topskip}{0in}        %\topskip: between header and text
\setlength{\headsep}{0in}
\setlength{\textheight}{692pt}   %\textheight: height of main text
\setlength{\textwidth}{8in}    % \textwidth: width of text
\setlength{\oddsidemargin}{-0.7in}  % \oddsidemargin: odd page left margin
\setlength{\evensidemargin}{0in} %\evensidemargin : even page left margin
\setlength{\parindent}{0.25in}   %\parindent: indentation of paragraphs
\setlength{\parskip}{0pt}        %\parskip: gap between paragraphs
\setlength{\voffset}{0.5in}

% Useful commands:

% \hfill    aligns-right everything right of \hfill

\begin{document}
\doublespacing
\title{Plasma Disruption 1D solution}
\author{C. Kawczynski \\
Department of Mechanical and Aerospace Engineering \\
University of California Los Angeles, USA\\
}
\maketitle

\section{Decoupling of 1D plasma-disruption governing equations}
In this document, decouple the 1D plasma disruption governing equations
\begin{equation}\begin{aligned}
u''   = - \frac{1}{\rho \nu \M} B_z^0 B_x' \\
B_x'' = \sigma \M (\PD_t B_x^0 - B_z^0 u') \\
\end{aligned} \end{equation}
Let
\begin{equation}\begin{aligned}
A = \frac{1}{\rho \nu \M} B_z^0, \qquad
C = \sigma \M \PD_t B_x^0, \qquad
D = \sigma \M B_z^0
\end{aligned} \end{equation}
\begin{equation}\begin{aligned}
u''   = - A B_x' \\
B_x'' = C - D u' \\
\end{aligned} \end{equation}

\section{Variable seperation transformation}
We may apply the transformation
\begin{equation}\begin{aligned}
X = u + F B_x \\
Y = u - F B_x \\
\end{aligned} \end{equation}

\subsection{Transformation for X}
We have
\begin{equation}\begin{aligned}
(X - F B_x)''   = - A B_x' \\
B_x'' = C - D (X - F B_x)' \\
\end{aligned} \end{equation}
Distributing
\begin{equation}\begin{aligned}
X'' - F B_x''   = - A B_x' \\
B_x'' = C - D X' + D F B_x' \\
\end{aligned} \end{equation}
Combining with factor $E$ for second equation
\begin{equation}\begin{aligned}
X'' - F B_x'' + FB_x''   = - A B_x' + E(C - D X' + D F B_x') \\
\end{aligned} \end{equation}
To ensure $B_x$ dissappears, we must enforce
\begin{equation}\begin{aligned}
-F + E = 0, \qquad E = F \\
-A + FDE = 0,\qquad E^2D = A, \qquad E = F = \sqrt{\frac{A}{D}}\\
\end{aligned} \end{equation}
So we have
\begin{equation}\begin{aligned}
X'' - F B_x'' + FB_x''   = - A B_x' + E(C - D X' + D F B_x') \\
X'' = - A B_x' + FC - FD X' + E^2 D B_x' \\
X'' = FC - FD X' + (E^2 D B_x' - A B_x') \\
X'' = FC - FD X' + \left(\frac{A}{D} D B_x' - A B_x' \right) \\
X'' = FC - FD X' \\
\end{aligned} \end{equation}
\subsection{Transformation for Y}
Reminder
\begin{equation}\begin{aligned}
u''   = - A B_x' \\
B_x'' = C - D u' \\
\end{aligned} \end{equation}
We have
\begin{equation}\begin{aligned}
(Y + F B_x)''   = - A B_x' \\
B_x'' = C - D (Y + F B_x)' \\
\end{aligned} \end{equation}
Distributing
\begin{equation}\begin{aligned}
Y'' + F B_x''   = - A B_x' \\
B_x'' = C - D Y' - D F B_x' \\
\end{aligned} \end{equation}
Combining with factor $-E$ for second equation yields
\begin{equation}\begin{aligned}
Y'' + F B_x'' - FB_x''   = - A B_x' - E(C - D Y' - D F B_x') \\
Y'' = - A B_x' - FC + E D Y' + E D F B_x' \\
Y'' = - FC + E D Y' + (E D F B_x' - A B_x') \\
Y'' = - FC + E D Y' + \left(\frac{A}{D} D B_x' - A B_x' \right) \\
Y'' = - FC + F D Y' \\
\end{aligned} \end{equation}
\section{Transformation summary}
Our decoupled equations are
\begin{equation}\begin{aligned}
X'' + F D X' =   FC \\
Y'' - F D Y' = - FC \\
\end{aligned} \end{equation}
Where
\begin{equation}\begin{aligned}
A = \frac{1}{\rho \nu \M} B_z^0, \qquad
C = \sigma \M \PD_t B_x^0, \qquad
D = \sigma \M B_z^0, \qquad
F = \sqrt{\frac{A}{D}} \\
\end{aligned} \end{equation}
With transformations
\begin{equation}\begin{aligned}
X = u + F B_x \\
Y = u - F B_x \\
\end{aligned} \end{equation}
And inverse transformations
\begin{equation}\begin{aligned}
u   = \frac{1}{2} \left( X + Y \right) \\
B_x = \frac{1}{2E} \left( X - Y \right) \\
\end{aligned} \end{equation}
\begin{equation}\begin{aligned}
A = \frac{1}{\rho \nu \M} B_z^0, \qquad
C = \sigma \M \PD_t B_x^0, \qquad
D = \sigma \M B_z^0, \qquad
F = \sqrt{\frac{A}{D}} \\
\end{aligned} \end{equation}


\end{document}