\documentclass[11pt]{article}
% \documentclass[3p,twocolumn,10pt]{elsarticle}
\usepackage{graphicx}    % needed for including graphics e.g. EPS, PS
\usepackage{epstopdf}
\usepackage{amsmath}
\usepackage{amssymb}
\usepackage{hyperref}
\usepackage{xspace}
\usepackage{mathtools}
\usepackage{tikz}
\usepackage{epsfig}
\usepackage{float}
%\usepackage{natbib}
\usepackage{subfigure}
\usepackage{setspace}
\usepackage{tabularx,ragged2e,booktabs,caption}

\usepackage{xcolor}
\usepackage{xspace}
\usepackage{longtable}
\usepackage{mathtools}
\usepackage{natbib}
\usepackage{setspace}
\usepackage{ragged2e}
\usepackage{etoolbox}
\usepackage{geometry}

\input{../../../useful_commands.tex}

\newcommand{\volume}{\mathop{\ooalign{\hfil$V$\hfil\cr\kern0.08em--\hfil\cr}}\nolimits}
\newcommand{\figWidth}{0.45\textwidth}
\newcommand{\figSuffix}{_png.png}
\newcommand{\pushright}[1]{\ifmeasuring@#1\else\omit\hfill$\displaystyle#1$\fi\ignorespaces}
\newcommand{\hfillMath}{\hskip \textwidth minus \textwidth}

\setlength{\oddsidemargin}{0.1in}
\setlength{\textwidth}{7.25in}

\setlength{\topmargin}{-1in}     %\topmargin: gap above header
\setlength{\headheight}{0in}     %\headheight: height of header
\setlength{\topskip}{0in}        %\topskip: between header and text
\setlength{\headsep}{0in}
\setlength{\textheight}{692pt}   %\textheight: height of main text
\setlength{\textwidth}{8in}    % \textwidth: width of text
\setlength{\oddsidemargin}{-0.7in}  % \oddsidemargin: odd page left margin
\setlength{\evensidemargin}{0in} %\evensidemargin : even page left margin
\setlength{\parindent}{0.25in}   %\parindent: indentation of paragraphs
\setlength{\parskip}{0pt}        %\parskip: gap between paragraphs
\setlength{\voffset}{0.5in}

% Useful commands:

% \hfill    aligns-right everything right of \hfill

\begin{document}
\doublespacing
\title{Plasma Disruption 2D solution}
\author{C. Kawczynski \\
Department of Mechanical and Aerospace Engineering \\
University of California Los Angeles, USA\\
}
\maketitle

\section{Solving Shercliff-modified governing equations}
In this document, we attempt the solution to the decoupled equations
\begin{equation}\begin{aligned}
\DEL^2 X + A \PD_x X = - C, \qquad \text{BCs: $X = 0 $ on $\PD \Omega$} \\
\DEL^2 Y - A \PD_x Y = - D, \qquad \text{BCs: $Y = 0 $ on $\PD \Omega$} \\
\end{aligned} \end{equation}
Where constant $A$ is assumed to be positive. We assume the solution is the sum of a homogeneous equation, where $C,D$, are neglected, plus a solution with the coefficients present.
\begin{equation}\begin{aligned}
X = X_h(x,y) + X_p(y) \\
Y = Y_h(x,y) + Y_p(y) \\
\end{aligned} \end{equation}
\begin{equation}\begin{aligned}
\DEL^2 X_h + A \PD_x X_h = 0, \qquad\qquad \DEL^2 X_p = -C \\
\DEL^2 Y_h - A \PD_x Y_h = 0, \qquad\qquad \DEL^2 Y_p = -D \\
\end{aligned} \end{equation}

\section{Homogeneous solution for X}
Governing equation
\begin{equation}\begin{aligned}
\DEL^2 X_h + A \PD_x X_h = 0, \qquad\qquad X_h = X_h(x,y) \\
\end{aligned} \end{equation}
Assume the solution is separable:
\begin{equation}\begin{aligned}
X_h(x,y) = F(x)G(y) \\
\end{aligned} \end{equation}
Governing equation becomes
\begin{equation}\begin{aligned}
G F'' + FG'' + A G F' = 0 \\
 \frac{F''}{F} + \frac{G''}{G} + A \frac{F'}{F} = 0 \\
 \frac{F''}{F} + A \frac{F'}{F} = - \frac{G''}{G} = \lambda \\
\end{aligned} \end{equation}

\noindent\begin{minipage}[b]{.5\linewidth}\centering
\begin{equation}\begin{aligned}
\frac{F''}{F} + A \frac{F'}{F} = \lambda \\
F'' + A F' - F \lambda = 0 \\
F = \alpha e^{\gamma x} \\
\gamma^2 + A \gamma - \lambda = 0 \\
\gamma_{1,2} = -A \pm \frac{\sqrt{A^2 + 4\lambda}}{2} \\
F_n = \alpha_1 e^{\left(-A + \frac{\sqrt{A^2 + 4\lambda}}{2}\right) x} + \alpha_2 e^{\left(-A - \frac{\sqrt{A^2 + 4\lambda}}{2} \right) x} \\
F_n(0) = \alpha_1 + \alpha_2  = 0 \\
\alpha_2 = - \alpha_1 \\
F_n = \alpha_1 \left( e^{\left(-A + \frac{\sqrt{A^2 + 4\lambda_n}}{2}\right) x} - e^{\left(-A - \frac{\sqrt{A^2 + 4\lambda_n}}{2} \right) x} \right) \\
F_n = \alpha_1 e^{-A} 2 \sinh \left( \left[\frac{\sqrt{A^2 + \left(2 n \pi \frac{L}{b} \right)^2}}{2}\right] x \right) \\
\end{aligned} \end{equation}
\end{minipage}
\noindent\begin{minipage}[b]{.5\linewidth}\centering
\begin{equation}\begin{aligned}
\frac{G''}{G} = - \lambda \\
G'' + G \lambda = 0 \\
G = \beta e^{\theta y} \\
\theta^2 + \lambda = 0 \\
\theta_{1,2} = \pm i \sqrt{\lambda} \\
G = \beta_1 e^{i \sqrt{\lambda} y} + \beta_2 e^{-i \sqrt{\lambda} y} \\
G(0) = \beta_1 + \beta_2 = 0 \\
\beta_2 = - \beta_1 \\
G = \beta_1 \left( e^{i \sqrt{\lambda} y} - e^{-i \sqrt{\lambda} y} \right) \\
G(b/L) = \beta_1 \left( e^{i \sqrt{\lambda} b/L} - e^{-i \sqrt{\lambda} b/L} \right) = 0 \\
                 \left( e^{2 i \sqrt{\lambda} b/L} - 1 \right) = 0 \\
2 i \sqrt{\lambda_n} b/L = \pi i 2n, \qquad n = 0,1,2,3,... \\
\lambda_n = \left( n \pi \frac{L}{b} \right)^2 \\
G_n = \beta_1 \left( e^{i n \pi \frac{L}{b} y} - e^{-i n \pi \frac{L}{b} y} \right) \\
G_n = 2i \beta_1 \sin \left(n \pi \frac{L}{b} y \right) \\
\end{aligned} \end{equation}
\end{minipage}
Our general solution to the homogeneous solution is then
\begin{equation}\begin{aligned}
X_h = \sum_{n=1}^{\infty} \zeta_n \sinh \left( \left[\frac{\sqrt{A^2 + \left(2 n \pi \frac{L}{b} \right)^2}}{2}\right] x \right) \sin \left(n \pi \frac{L}{b} y \right) \\
\end{aligned} \end{equation}

\section{Homogeneous solution for Y}
Governing equation
\begin{equation}\begin{aligned}
\DEL^2 Y_h - A \PD_x Y_h = 0, \qquad\qquad Y_h = Y_h(x,y) \\
\end{aligned} \end{equation}
Assume the solution is separable:
\begin{equation}\begin{aligned}
Y_h(x,y) = F(x)G(y) \\
\end{aligned} \end{equation}
\begin{equation}\begin{aligned}
G F'' + FG'' - A G F' = 0 \\
 \frac{F''}{F} + \frac{G''}{G} - A \frac{F'}{F} = 0 \\
 \frac{F''}{F} - A \frac{F'}{F} = - \frac{G''}{G} = \lambda \\
\end{aligned} \end{equation}

\noindent\begin{minipage}[b]{.5\linewidth}\centering
\begin{equation}\begin{aligned}
\frac{F''}{F} - A \frac{F'}{F} = \lambda \\
F'' - A F' - F \lambda = 0 \\
F = \alpha e^{\gamma x} \\
\gamma^2 - A \gamma - \lambda = 0 \\
\gamma_{1,2} = A \pm \frac{\sqrt{A^2 + 4\lambda}}{2} \\
F_n = \alpha_1 e^{\left(A + \frac{\sqrt{A^2 + 4\lambda}}{2}\right) x} + \alpha_2 e^{\left(A - \frac{\sqrt{A^2 + 4\lambda}}{2} \right) x} \\
F_n(0) = \alpha_1 + \alpha_2  = 0 \\
\alpha_2 = - \alpha_1 \\
F_n = \alpha_1 \left( e^{\left(A + \frac{\sqrt{A^2 + 4\lambda_n}}{2}\right) x} - e^{\left(A - \frac{\sqrt{A^2 + 4\lambda_n}}{2} \right) x} \right) \\
F_n = \alpha_1 e^{A} 2 \sinh \left( \left[\frac{\sqrt{A^2 + \left(2 n \pi \frac{L}{b} \right)^2}}{2}\right] x \right) \\
\end{aligned} \end{equation}
\end{minipage}
\noindent\begin{minipage}[b]{.5\linewidth}\centering
\begin{equation}\begin{aligned}
\frac{G''}{G} = - \lambda \\
G'' + G \lambda = 0 \\
G = \beta e^{\theta y} \\
\theta^2 + \lambda = 0 \\
\theta_{1,2} = \pm i \sqrt{\lambda} \\
G = \beta_1 e^{i \sqrt{\lambda} y} + \beta_2 e^{-i \sqrt{\lambda} y} \\
G(0) = \beta_1 + \beta_2 = 0 \\
\beta_2 = - \beta_1 \\
G = \beta_1 \left( e^{i \sqrt{\lambda} y} - e^{-i \sqrt{\lambda} y} \right) \\
G(b/L) = \beta_1 \left( e^{i \sqrt{\lambda} b/L} - e^{-i \sqrt{\lambda} b/L} \right) = 0 \\
                 \left( e^{2 i \sqrt{\lambda} b/L} - 1 \right) = 0 \\
2 i \sqrt{\lambda_n} b/L = \pi i 2n, \qquad n = 0,1,2,3,... \\
\lambda_n = \left( n \pi \frac{L}{b} \right)^2 \\
G_n = \beta_1 \left( e^{i n \pi \frac{L}{b} y} - e^{-i n \pi \frac{L}{b} y} \right) \\
G_n = 2i \beta_1 \sin \left(n \pi \frac{L}{b} y \right) \\
\end{aligned} \end{equation}
\end{minipage}
Our general solution to the homogeneous solution is then
\begin{equation}\begin{aligned}
Y_h = \sum_{n=1}^{\infty} \Phi_n \sinh \left( \left[\frac{\sqrt{A^2 + \left(2 n \pi \frac{L}{b} \right)^2}}{2}\right] x \right) \sin \left(n \pi \frac{L}{b} y \right) \\
\end{aligned} \end{equation}

\section{Homogeneous solution summary}
\begin{equation}\begin{aligned}
X_h = \sum_{n=1}^{\infty} \zeta_n \sinh \left( \left[\frac{\sqrt{A^2 + \left(2 n \pi \frac{L}{b} \right)^2}}{2}\right] x \right) \sin \left(n \pi \frac{L}{b} y \right) \\
\end{aligned} \end{equation}
\begin{equation}\begin{aligned}
Y_h = \sum_{n=1}^{\infty} \Phi_n \sinh \left( \left[\frac{\sqrt{A^2 + \left(2 n \pi \frac{L}{b} \right)^2}}{2}\right] x \right) \sin \left(n \pi \frac{L}{b} y \right) \\
\end{aligned} \end{equation}

\section{Non-homogeneous solution}
Governing equation
\begin{equation}\begin{aligned}
\DEL^2 X_p = -C, \qquad X_p = X_p(y) \\
\DEL^2 Y_p = -D, \qquad Y_p = Y_p(y) \\
\end{aligned} \end{equation}
The solution only depends on $y$:
\begin{equation}\begin{aligned}
X_p'' = -C \\
Y_p'' = -D \\
\end{aligned} \end{equation}
So integration is trivially performed. First integration yields
\begin{equation}\begin{aligned}
X_p' = -C y + c_1 \\
Y_p' = -D y + b_1 \\
\end{aligned} \end{equation}
Second integration yields
\begin{equation}\begin{aligned}
X_p = -C \frac{1}{2} y^2 + c_1 y + c_2 \\
Y_p = -D \frac{1}{2} y^2 + b_1 y + b_2 \\
\end{aligned} \end{equation}
Applying BCs, we have:
\begin{equation}\begin{aligned}
X_p(0) = 0 = c_2 \\
Y_p(0) = 0 = b_2 \\
X_p(b/L) = 0 = -C \frac{1}{2} (b/L)^2 + c_1 (b/L) \\
Y_p(b/L) = 0 = -D \frac{1}{2} (b/L)^2 + b_1 (b/L) \\
c_1 = \frac{L}{b} C \frac{1}{2} (b/L)^2 = \frac{b C}{2L} \\
b_1 = \frac{L}{b} D \frac{1}{2} (b/L)^2 = \frac{b D}{2L} \\
\end{aligned} \end{equation}
The particular solution is then
\begin{equation}\begin{aligned}
X_p = -C \frac{1}{2} y^2 + \frac{b C}{2L} y \\
Y_p = -D \frac{1}{2} y^2 + \frac{b D}{2L} y \\
\end{aligned} \end{equation}
Or
\begin{equation}\begin{aligned}
X_p = \frac{C y}{2} \left(\frac{b}{L} - y \right) \\
Y_p = \frac{D y}{2} \left(\frac{b}{L} - y \right) \\
\end{aligned} \end{equation}

\section{Total solution}
The total general solution is therefore:
\begin{equation}\begin{aligned}
X = \frac{C y}{2} \left(\frac{b}{L} - y \right) + \sum_{n=1}^{\infty} \zeta_n \sinh \left( \left[\frac{\sqrt{A^2 + \left(2 n \pi \frac{L}{b} \right)^2}}{2}\right] x \right) \sin \left(n \pi \frac{L}{b} y \right) \\
Y = \frac{D y}{2} \left(\frac{b}{L} - y \right) + \sum_{n=1}^{\infty} \Phi_n  \sinh \left( \left[\frac{\sqrt{A^2 + \left(2 n \pi \frac{L}{b} \right)^2}}{2}\right] x \right) \sin \left(n \pi \frac{L}{b} y \right) \\
\end{aligned} \end{equation}
Finally, the BC at $x=a/L$ must be applied:
\begin{equation}\begin{aligned}
X(a/L,y) = \frac{C y}{2} \left(\frac{b}{L} - y \right) + \sum_{n=1}^{\infty} \zeta_n \sinh \left( \left[\frac{\sqrt{A^2 + \left(2 n \pi \frac{L}{b} \right)^2}}{2}\right] (a/L) \right) \sin \left(n \pi \frac{L}{b} y \right) = 0 \\
Y(a/L,y) = \frac{D y}{2} \left(\frac{b}{L} - y \right) + \sum_{n=1}^{\infty} \Phi_n  \sinh \left( \left[\frac{\sqrt{A^2 + \left(2 n \pi \frac{L}{b} \right)^2}}{2}\right] (a/L) \right) \sin \left(n \pi \frac{L}{b} y \right) = 0 \\
\end{aligned} \end{equation}
Or
\begin{equation}\begin{aligned}
\sum_{n=1}^{\infty} \zeta_n \sinh \left( \left[\sqrt{A^2 + \left(2 n \pi \frac{L}{b} \right)^2}\right] \frac{a}{2L} \right) \sin \left(n \pi \frac{L}{b} y \right) = \frac{C y}{2} \left(y - \frac{b}{L}\right) \\
\sum_{n=1}^{\infty} \Phi_n  \sinh \left( \left[\sqrt{A^2 + \left(2 n \pi \frac{L}{b} \right)^2}\right] \frac{a}{2L} \right) \sin \left(n \pi \frac{L}{b} y \right) = \frac{D y}{2} \left(y - \frac{b}{L}\right) \\
\end{aligned} \end{equation}
Let
\begin{equation}\begin{aligned}
K_n = \sinh \left( \left[\sqrt{A^2 + \left(2 n \pi \frac{L}{b} \right)^2}\right] \frac{a}{2L} \right) \\
\end{aligned} \end{equation}
Then we have
\begin{equation}\begin{aligned}
\sum_{n=1}^{\infty} \zeta_n K_n \sin \left(n \pi \frac{L}{b} y \right) = \frac{C y}{2} \left(y - \frac{b}{L}\right) \\
\sum_{n=1}^{\infty} \Phi_n  K_n \sin \left(n \pi \frac{L}{b} y \right) = \frac{D y}{2} \left(y - \frac{b}{L}\right) \\
\end{aligned} \end{equation}
Quick aside

\noindent \rule{\textwidth}{1pt}
Fourier series coefficients over the domain $[0,L]$
\begin{equation}\begin{aligned}
f(x) = \frac{A_0}{2} + \sum_{n=1}^{\infty} \left[ A_n \cos\left( \frac{n \pi x}{L} \right) + B_n \sin\left( \frac{n \pi x}{L} \right) \right] \\
\end{aligned} \end{equation}
may be solved using
\begin{equation}\begin{aligned}
A_0 = \frac{2}{L} \int_0^L f(x) dx, \qquad
A_n = \frac{2}{L} \int_0^L f(x) \cos\left( \frac{n \pi x}{L} \right) dx, \qquad
B_n = \frac{2}{L} \int_0^L f(x) \sin\left( \frac{n \pi x}{L} \right) dx
\end{aligned} \end{equation}
\noindent \rule{\textwidth}{1pt}

These are sine series expansions with respect to $y$, whose coefficients may be found from
\begin{equation}\begin{aligned}
\zeta_n K_n = \frac{2L}{b} \int_0^{b/L} \frac{C y}{2} \left(y - \frac{b}{L}\right) \sin\left( n \pi \frac{b}{L}y \right) dy \\
\Phi_n  K_n = \frac{2L}{b} \int_0^{b/L} \frac{D y}{2} \left(y - \frac{b}{L}\right) \sin\left( n \pi \frac{b}{L}y \right) dy \\
\end{aligned} \end{equation}
Solving for $\zeta_n,\Phi_n$, we have
\begin{equation}\begin{aligned}
\zeta_n = \frac{1}{K_n} \frac{2L}{b} \int_0^{b/L} \frac{C y}{2} \left(y - \frac{b}{L}\right) \sin\left( n \pi \frac{b}{L}y \right) dy \\
\Phi_n  = \frac{1}{K_n} \frac{2L}{b} \int_0^{b/L} \frac{D y}{2} \left(y - \frac{b}{L}\right) \sin\left( n \pi \frac{b}{L}y \right) dy \\
\end{aligned} \end{equation}
Simplifying a bit
\begin{equation}\begin{aligned}
\zeta_n = C \frac{1}{K_n} \frac{L}{b} \int_0^{b/L} y \left(y - \frac{b}{L}\right) \sin\left( n \pi \frac{b}{L}y \right) dy \\
\Phi_n  = D \frac{1}{K_n} \frac{L}{b} \int_0^{b/L} y \left(y - \frac{b}{L}\right) \sin\left( n \pi \frac{b}{L}y \right) dy \\
\end{aligned} \end{equation}
Integration yields
\begin{equation}\begin{aligned}
I_n=\frac{2 L^3  \left( -1+\cos \left( \frac{b^2 n \pi}{L^2} \right) \right) +b^2 L n \pi \sin \left( \frac{b^2 n \pi}{L^2} \right) }{b^3 n^3 \pi^3}
\end{aligned} \end{equation}
So we have
\begin{equation}\begin{aligned}
\zeta_n = C \frac{1}{K_n} \frac{L}{b} I_n \\
\Phi_n  = D \frac{1}{K_n} \frac{L}{b} I_n \\
\end{aligned} \end{equation}

Returning to our total solution, we have

\begin{equation}\begin{aligned}
X = \frac{C y}{2} \left(\frac{b}{L} - y \right) + \sum_{n=1}^{\infty} C \frac{1}{K_n} \frac{L}{b} I_n \sinh \left( \left[\frac{\sqrt{A^2 + \left(2 n \pi \frac{L}{b} \right)^2}}{2}\right] x \right) \sin \left(n \pi \frac{L}{b} y \right) \\
Y = \frac{D y}{2} \left(\frac{b}{L} - y \right) + \sum_{n=1}^{\infty} D \frac{1}{K_n} \frac{L}{b} I_n \sinh \left( \left[\frac{\sqrt{A^2 + \left(2 n \pi \frac{L}{b} \right)^2}}{2}\right] x \right) \sin \left(n \pi \frac{L}{b} y \right) \\
\end{aligned} \end{equation}
Where
\begin{equation}\begin{aligned}
I_n=\frac{2 L^3  \left( -1+\cos \left( \frac{b^2 n \pi}{L^2} \right) \right) +b^2 L n \pi \sin \left( \frac{b^2 n \pi}{L^2} \right) }{b^3 n^3 \pi^3} \\
K_n = \sinh \left( \left[\sqrt{A^2 + \left(2 n \pi \frac{L}{b} \right)^2}\right] \frac{a}{2L} \right) \\
-Re \PD_z p = k \\
A = Ha B_x^0 \\
C = k - Ha \PD_t B_z^0 \\
D = k + Ha \PD_t B_z^0 \\
\end{aligned} \end{equation}
Solutions are reconstructed using:
\begin{equation}\begin{aligned}
w   =                 \frac{1}{2} (X + Y)\\
B_z = \frac{Re_m}{Ha} \frac{1}{2} (X - Y)\\
\end{aligned} \end{equation}


\end{document}